refactor to sigma eliminator

IMLTT/untyped/AbstractSyntax.lean
@@ -15,8 +15,7 @@ inductive Tm : Nat → Type where
   | lam : Tm n → Tm (n + 1) → Tm n
   | app : Tm n → Tm n → Tm n
   | pairSigma : Tm n → Tm n → Tm n
-  | firstSigma : Tm n → Tm n
-  | secondSigma : Tm n → Tm n
+  | indSigma: Tm n → Tm (n + 1) → Tm (n + 1) → Tm (n + 2) → Tm n → Tm n
   | zeroNat : Tm n
   | succNat : Tm n → Tm n
   | indNat : Tm (n + 1) → Tm n → Tm (n + 2) → Tm n → Tm n
@@ -41,8 +40,6 @@ notation:max "⋆" => Tm.tt
 notation:98 "λ" A "; " b => Tm.lam A b
 infixl:98 "◃" => Tm.app
 infixl:98 "&" => Tm.pairSigma -- FIXME: add ()
-prefix:98 "π₁" => Tm.firstSigma
-prefix:98 "π₂" => Tm.secondSigma
 notation:max "𝓏" => Tm.zeroNat
 notation:max "𝓈(" x ")" => Tm.succNat x
 
