IMLTT/typed/SigmaProjections.lean
@@ -1,0 +1,101 @@
+import IMLTT.untyped.AbstractSyntax
+import IMLTT.untyped.Weakening
+import IMLTT.untyped.Substitution
+
+import IMLTT.typed.JudgmentsAndRules
+import IMLTT.typed.proofs.admissable.Weakening
+import IMLTT.typed.proofs.admissable.Substitution
+import IMLTT.typed.proofs.admissable.WeakSubstitution.WeakSubstitution
+import IMLTT.typed.proofs.admissable.Inversion
+import IMLTT.typed.proofs.admissable.FunctionalityTyping
+import IMLTT.typed.proofs.admissable.ContextConv
+
+import IMLTT.typed.proofs.boundary.BoundaryTypesTerms
+
+#check HasType.sigma_elim
+-- TODO: first eliminator then computions
+
+theorem this_might_work :
+    A⌊↑ₚidₚ⌋⌊↑ₚidₚ⌋ =  A⌊↑ₚidₚ⌋⌈(ₛ↑ₚ↑ₚidₚ), v(1)&v(0)⌉ :=
+  by
+    simp [substitution_comp_σρ]
+    simp [comp_substitute_weaken]
+    simp [weakening_comp]
+    simp [comp_weaken]
+    apply Eq.symm
+    apply conversion_sub_weak
+
+theorem sigma_elim_proj_first :
+    ∃a, Γ ⊢ ΣA;B type → (Γ ⊢ p ∶ ΣA;B) → Γ ⊢ a ∶ A :=
+  by
+    apply Exists.intro
+    intro hSi hpSi
+    have h := sigma_is_type_inversion hSi
+    have C := weakening_type (And.left h) hSi
+    have c : (Γ ⬝ A ⬝ B ⊢ v(0)⌊↑ₚidₚ⌋ ∶ A⌊↑ₚidₚ⌋⌊↑ₚidₚ⌋) :=
+        by
+          apply HasType.weak
+          · apply HasType.var
+            apply And.left h
+          · apply And.right h
+    rw [this_might_work] at c
+    have ind := HasType.sigma_elim hpSi C c
+    rw [substitution_shift_substitute_zero] at ind
+    apply ind
+
+def sigma_elim_π₁ (Si : Γ ⊢ ΣA;B type) (pSi : Γ ⊢ p ∶ ΣA;B) : Γ ⊢ A.indSigma B (A⌊↑ₚidₚ⌋) (v(0)⌊↑ₚidₚ⌋) p ∶ A :=
+  have h := sigma_is_type_inversion Si
+  have C := weakening_type (And.left h) Si
+  have c : (Γ ⬝ A ⬝ B ⊢ v(0)⌊↑ₚidₚ⌋ ∶ A⌊↑ₚidₚ⌋⌈(ₛ↑ₚ↑ₚidₚ), v(1)&v(0)⌉) :=
+      by
+        rw [←this_might_work]
+        apply HasType.weak
+        · apply HasType.var
+          apply And.left h
+        · apply And.right h
+  have ind : Γ ⊢ A.indSigma B (A⌊↑ₚidₚ⌋) (v(0)⌊↑ₚidₚ⌋) p ∶ A := 
+    by
+      have h := HasType.sigma_elim pSi C c
+      rw [substitution_shift_substitute_zero] at h
+      apply h
+  ind
+
+theorem sigma_comp_proj_first :
+    ∀a b, Γ ⊢ ΣA;B type → (Γ ⊢ a&b ∶ ΣA;B) → Γ ⊢ a ∶ A :=
+  by
+    intro a b
+    intro hSi hpSi
+    have h := sigma_is_type_inversion hSi
+    have C := weakening_type (And.left h) hSi
+    have c : (Γ ⬝ A ⬝ B ⊢ v(0)⌊↑ₚidₚ⌋ ∶ A⌊↑ₚidₚ⌋⌊↑ₚidₚ⌋) := -- C⌈(ₛ↑ₚ↑ₚidₚ), v(1)&v(0)⌉)
+        by
+          apply HasType.weak
+          · apply HasType.var
+            apply And.left h
+          · apply And.right h
+    rw [this_might_work] at c
+    sorry
+    -- have ind := IsEqualTerm.sigma_comp sorry sorry C c
+    -- rw [substitution_shift_substitute_zero] at ind
+    -- apply ind
+
+theorem sigma_elim_proj_second :
+    ∃b, (Γ ⊢ p ∶ ΣA;B) → Γ ⊢ b ∶ B⌈a⌉₀  := -- how to correctly express a?
+  by
+    apply Exists.intro
+    intro hpSi
+    have hSi := boundary_term_type hpSi
+    have h := sigma_is_type_inversion hSi
+    have C := weakening_type (And.left h) hSi
+    have c : (Γ ⬝ A ⬝ B ⊢ v(0)⌊↑ₚidₚ⌋ ∶ A⌊↑ₚidₚ⌋⌊↑ₚidₚ⌋) := -- C⌈(ₛ↑ₚ↑ₚidₚ), v(1)&v(0)⌉)
+        by
+          apply HasType.weak
+          · apply HasType.var
+            apply And.left h
+          · apply And.right h
+    rw [this_might_work] at c
+    have ind := HasType.sigma_elim hpSi C c
+    rw [substitution_shift_substitute_zero] at ind
+    any_goals sorry
+    -- apply ind
+
