IMLTT/typed/proofs/Recursor.lean
@@ -85,12 +85,15 @@ theorem judgment_recursor :
     (a_1 : Γ ⊢ f ∶ (.pi A B)) (a_2 : Γ ⊢ a ∶ A),
     motive_3 Γ f (.pi A B) a_1 → motive_3 Γ a A a_2 
     → motive_3 Γ (.app f a) (substitute_zero a B) (HasType.pi_elim a_1 a_2))
-  → (HasTypeSigmaFirst : ∀ {n : Nat} {Γ : Ctx n} {p A : Tm n} {B : Tm (n + 1)}
-    (a_1 : Γ ⊢ p ∶ (ΣA;B)), motive_3 Γ p (ΣA;B) a_1
-    → motive_3 Γ (π₁ p) A (HasType.sigma_first a_1))
-  → (HasTypeSigmaSecond : ∀ {n : Nat} {Γ : Ctx n} {p A : Tm n} {B : Tm (n + 1)}
-    (a_1 : Γ ⊢ p ∶ (ΣA;B)), motive_3 Γ p (ΣA;B) a_1
-    → motive_3 Γ (π₂ p) (B⌈π₁ p⌉₀) (HasType.sigma_second a_1))
+  → (HasTypeSigmaElim : ∀ {n : Nat} {Γ : Ctx n} {A : Tm n} {B : Tm (n + 1)} {p : Tm n} 
+    {C : Tm (n + 1)} {c : Tm (n + 1 + 1)}
+    (a_1 : Γ ⊢ p ∶ (.sigma A B)) (a_2 : (Γ ⬝ (.sigma A B)) ⊢ C type)
+    (a_3 : (Γ ⬝ A ⬝ B) ⊢ c ∶ (substitute (Subst.weak (.shift (.shift .id)), 
+      (.pairSigma v(1) v(0))) C)),
+    motive_3 Γ p (.sigma A B) a_1 → motive_2 (Γ ⬝ (.sigma A B)) C a_2
+    → motive_3 (Γ ⬝ A ⬝ B) c
+      (substitute (Subst.weak (.shift (.shift .id)), (.pairSigma v(1) v(0))) C) a_3
+    → motive_3 Γ (.indSigma A B C c p) (substitute_zero p C) (HasType.sigma_elim a_1 a_2 a_3) )
   → (HasTypeNatElim : ∀ {n : Nat} {Γ : Ctx n} {z x : Tm n} {A : Tm (n + 1)} {s : Tm (n + 2)}
     (a_1 : Γ ⬝ 𝒩  ⊢ A type) (a_2 : Γ ⊢ z ∶ A⌈𝓏⌉₀) 
     (a_3 : (Γ ⬝ 𝒩 ⬝ A) ⊢ s ∶ (A⌈(ₛ↑ₚidₚ), 𝓈(v(0))⌉⌊↑ₚidₚ⌋))
@@ -156,14 +159,14 @@ theorem judgment_recursor :
     (a_1 : (Γ ⬝ A) ⊢ b ∶ B) (a_2 : Γ ⊢ a ∶ A), motive_3 (Γ ⬝ A) b B a_1 → motive_3 Γ a A a_2 
     → motive_5 Γ ((A.lam b).app a) (substitute_zero a b) (substitute_zero a B) 
       (IsEqualTerm.pi_comp a_1 a_2))
-  → (IsEqualTermSigmaFirstComp : ∀ {n : Nat} {Γ : Ctx n} {a b A : Tm n} {B : Tm (n + 1)}
-    (a_1 : Γ ⊢ a ∶ A) (a_2 : Γ ⊢ b ∶ B⌈a⌉₀) (a_3 : Γ ⊢ (ΣA;B) type), 
-    motive_3 Γ a A a_1 → motive_3 Γ b (B⌈a⌉₀) a_2 → motive_2 Γ (ΣA;B) a_3
-    → motive_5 Γ (π₁ (.pairSigma a b)) a A (IsEqualTerm.sigma_first_comp a_1 a_2 a_3))
-  → (IsEqualTermSigmaSecondComp : ∀ {n : Nat} {Γ : Ctx n} {a b A : Tm n} {B : Tm (n + 1)}
-    (a_1 : Γ ⊢ a ∶ A) (a_2 : Γ ⊢ b ∶ B⌈a⌉₀) (a_3 : Γ ⊢ (ΣA;B) type), 
-    motive_3 Γ a A a_1 → motive_3 Γ b (B⌈a⌉₀) a_2 → motive_2 Γ (ΣA;B) a_3
-    → motive_5 Γ (π₂ (.pairSigma a b)) b (B⌈π₁ a&b⌉₀) (IsEqualTerm.sigma_second_comp a_1 a_2 a_3))
+  → (IsEqualTermSigmaComp : ∀ {n : Nat} {Γ : Ctx n} {a A b : Tm n} {B C : Tm (n + 1)} 
+    {c : Tm (n + 1 + 1)} (a_1 : Γ ⊢ a ∶ A)
+    (a_2 : Γ ⊢ b ∶ substitute_zero a B) (a_3 : (Γ ⬝ A.sigma B) ⊢ C type)
+    (a_4 : (Γ ⬝ A ⬝ B) ⊢ c ∶ substitute (Subst.weak Weak.id.shift.shift, v(1).pairSigma v(0)) C),
+    motive_3 Γ a A a_1 → motive_3 Γ b (substitute_zero a B) a_2 → motive_2 (Γ ⬝ A.sigma B) C a_3 
+    → motive_3 (Γ ⬝ A ⬝ B) c (substitute (Subst.weak Weak.id.shift.shift, v(1).pairSigma v(0)) C) a_4 
+    → motive_5 Γ (A.indSigma B C c (a.pairSigma b)) (substitute (Subst.weak Weak.id, a, b) c)
+      (substitute_zero (a.pairSigma b) C) (IsEqualTerm.sigma_comp a_1 a_2 a_3 a_4))
   → (IsEqualTermNatZeroComp : ∀ {n : Nat} {Γ : Ctx n} {z : Tm n} {A : Tm (n + 1)} {s : Tm (n + 2)}
     (a_1 : Γ ⬝ 𝒩  ⊢ A type) (a_2 : Γ ⊢ z ∶ A⌈𝓏⌉₀)
     (a_3 : (Γ ⬝ 𝒩 ⬝ A) ⊢ s ∶ (A⌈(ₛ↑ₚidₚ), 𝓈(v(0))⌉⌊↑ₚidₚ⌋))
@@ -213,12 +216,16 @@ theorem judgment_recursor :
     (a_1 : Γ ⊢ a ≡ a' ∶ A) (a_2 : Γ ⊢ b ≡ b' ∶ substitute_zero a B) (a_3 : Γ ⬝ A ⊢ B type),
     motive_5 Γ a a' A a_1 → motive_5 Γ b b' (substitute_zero a B) a_2 → motive_2 (Γ ⬝ A) (B) a_3
     → motive_5 Γ (a.pairSigma b) (a'.pairSigma b') (A.sigma B) (IsEqualTerm.sigma_intro_eq a_1 a_2 a_3))
-  → (IsEqualTermSigmaFirstEq : ∀ {n : Nat} {Γ : Ctx n} {p p' A : Tm n} {B : Tm (n + 1)}
-    (a_1 : Γ ⊢ p ≡ p' ∶ (ΣA;B)), motive_5 Γ p p' (ΣA;B) a_1
-    → motive_5 Γ (π₁ p) (π₁ p') A (IsEqualTerm.sigma_first_eq a_1))
-  → (IsEqualTermSigmaSecondEq : ∀ {n : Nat} {Γ : Ctx n} {p p' A : Tm n} {B : Tm (n + 1)}
-    (a_1 : Γ ⊢ p ≡ p' ∶ (ΣA;B)), motive_5 Γ p p' (ΣA;B) a_1
-    → motive_5 Γ (π₂ p) (π₂ p') (B⌈π₁ p⌉₀) (IsEqualTerm.sigma_second_eq a_1))
+  → (IsEqualTermSigmaElimEq :  ∀ {n : Nat} {Γ : Ctx n} {A : Tm n} {B : Tm (n + 1)} {A' : Tm n} 
+    {B' : Tm (n + 1)} {p p' : Tm n} {C C' : Tm (n + 1)} {c c' : Tm (n + 1 + 1)} 
+    (a : Γ ⊢ A ≡ A' type) (a_4 : (Γ ⬝ A) ⊢ B ≡ B' type) (a_1 : Γ ⊢ p ≡ p' ∶ A.sigma B)
+    (a_2 : (Γ ⬝ A.sigma B) ⊢ C ≡ C' type)
+    (a_3 : (Γ ⬝ A ⬝ B) ⊢ c ≡ c' ∶ substitute (Subst.weak Weak.id.shift.shift, v(1).pairSigma v(0)) C),
+    motive_4 Γ A A' a → motive_4 (Γ ⬝ A) B B' a_4 → motive_5 Γ p p' (A.sigma B) a_1 
+    → motive_4 (Γ ⬝ A.sigma B) C C' a_2
+    → motive_5 (Γ ⬝ A ⬝ B) c c' (substitute (Subst.weak Weak.id.shift.shift, v(1).pairSigma v(0)) C) a_3
+    → motive_5 Γ (A.indSigma B C c p) (A'.indSigma B' C' c' p') (substitute_zero p C)
+      (IsEqualTerm.sigma_elim_eq a a_4 a_1 a_2 a_3))
   → (IsEqualTermNatZeroIntroEq : ∀ {n : Nat} {Γ : Ctx n}
     (a : Γ ctx), motive_1 Γ a → motive_5 Γ 𝓏 𝓏 𝒩  (IsEqualTerm.nat_zero_intro_eq a))
   → (IsEqualTermNatSuccIntroEq : ∀ {n : Nat} {Γ : Ctx n} {x x' : Tm n}
@@ -289,7 +296,7 @@ theorem judgment_recursor :
           hHasTypeNatZeroIntro hHasTypeNatSuccIntro hHasTypeIdenIntro
           hHasTypeUnivUnit hHasTypeUnivEmpty hHasTypeUnivPi hHasTypeUnivSigma
           hHasTypeUnivNat hHasTypeUnivIden
-          hHasTypeUnitElim hHasTypeEmptyElim hHasTypePiElim hHasTypeSigmaFirst hHasTypeSigmaSecond 
+          hHasTypeUnitElim hHasTypeEmptyElim hHasTypePiElim hHasTypeSigmaElim
           hHasTypeNatElim hHasTypeIdenElim
           hHasTypeTyConv
     intro hIsEqualTypeUnitFormEq hIsEqualTypeEmptyFormEQ hIsEqualTypePiFormEq hIsEqualTypeSigmaFormEq
@@ -297,11 +304,10 @@ theorem judgment_recursor :
           hIsEqualTypeIdenFormEq hIsEqalTypeUnivFormEq hIsEqualTypeUnivElimEq
           hIsEqualTypeTypeSymm hIsEqualTypeTypeTrans
     intro hIsEqualTermVarEq hIsEqualTermWeakEq hIsEqualTermUnitComp hIsEqualTermPiComp
-          hIsEqualTermSigmaFirstComp hIsEqualTermSigmaSecondComp
-          hIsEqualTermNatZeroComp hIsEqualTermNatSuccComp 
+          hIsEqualTermSigmaComp hIsEqualTermNatZeroComp hIsEqualTermNatSuccComp 
           hIsEqualTermIdenComp hIsEqualTermUnitIntroEq hIsEqualTermUnitElimEq hIsEqualTermEmptyElimEq
           hIsEqualTermPiIntroEq hIsEqualTermPiElimEq hIsEqualTermSigmaIntroEq
-          hIsEqualTermSigmaFirstEq hIsEqualTermSigmaSecondEq
+          hIsEqualTermSigmaElimEq
           hIsEqualTermNatZeroIntroEq hIsEqualTermNatSuccIntroEq
           hIsEqualTermNatElimEq
           hIsEqualTermIdenIntroEq hIsEqualTermIdenElimEq hIsEqualTermUnivUnitEq
@@ -322,7 +328,7 @@ theorem judgment_recursor :
           hHasTypeNatZeroIntro hHasTypeNatSuccIntro hHasTypeIdenIntro
           hHasTypeUnivUnit hHasTypeUnivEmpty hHasTypeUnivPi hHasTypeUnivSigma
           hHasTypeUnivNat hHasTypeUnivIden
-          hHasTypeUnitElim hHasTypeEmptyElim hHasTypePiElim hHasTypeSigmaFirst hHasTypeSigmaSecond 
+          hHasTypeUnitElim hHasTypeEmptyElim hHasTypePiElim hHasTypeSigmaElim
           hHasTypeNatElim hHasTypeIdenElim
           hHasTypeTyConv
         hIsEqualTypeUnitFormEq hIsEqualTypeEmptyFormEQ hIsEqualTypePiFormEq hIsEqualTypeSigmaFormEq
@@ -330,11 +336,10 @@ theorem judgment_recursor :
           hIsEqualTypeIdenFormEq hIsEqalTypeUnivFormEq hIsEqualTypeUnivElimEq
           hIsEqualTypeTypeSymm hIsEqualTypeTypeTrans
         hIsEqualTermVarEq hIsEqualTermWeakEq hIsEqualTermUnitComp hIsEqualTermPiComp
-          hIsEqualTermSigmaFirstComp hIsEqualTermSigmaSecondComp
-          hIsEqualTermNatZeroComp hIsEqualTermNatSuccComp 
+          hIsEqualTermSigmaComp hIsEqualTermNatZeroComp hIsEqualTermNatSuccComp 
           hIsEqualTermIdenComp hIsEqualTermUnitIntroEq hIsEqualTermUnitElimEq hIsEqualTermEmptyElimEq
           hIsEqualTermPiIntroEq hIsEqualTermPiElimEq hIsEqualTermSigmaIntroEq
-          hIsEqualTermSigmaFirstEq hIsEqualTermSigmaSecondEq
+          hIsEqualTermSigmaElimEq
           hIsEqualTermNatZeroIntroEq hIsEqualTermNatSuccIntroEq
           hIsEqualTermNatElimEq
           hIsEqualTermIdenIntroEq hIsEqualTermIdenElimEq hIsEqualTermUnivUnitEq
@@ -354,7 +359,7 @@ theorem judgment_recursor :
           hHasTypeNatZeroIntro hHasTypeNatSuccIntro hHasTypeIdenIntro
           hHasTypeUnivUnit hHasTypeUnivEmpty hHasTypeUnivPi hHasTypeUnivSigma
           hHasTypeUnivNat hHasTypeUnivIden
-          hHasTypeUnitElim hHasTypeEmptyElim hHasTypePiElim hHasTypeSigmaFirst hHasTypeSigmaSecond 
+          hHasTypeUnitElim hHasTypeEmptyElim hHasTypePiElim hHasTypeSigmaElim
           hHasTypeNatElim hHasTypeIdenElim
           hHasTypeTyConv
         hIsEqualTypeUnitFormEq hIsEqualTypeEmptyFormEQ hIsEqualTypePiFormEq hIsEqualTypeSigmaFormEq
@@ -362,11 +367,10 @@ theorem judgment_recursor :
           hIsEqualTypeIdenFormEq hIsEqalTypeUnivFormEq hIsEqualTypeUnivElimEq
           hIsEqualTypeTypeSymm hIsEqualTypeTypeTrans
         hIsEqualTermVarEq hIsEqualTermWeakEq hIsEqualTermUnitComp hIsEqualTermPiComp
-          hIsEqualTermSigmaFirstComp hIsEqualTermSigmaSecondComp
-          hIsEqualTermNatZeroComp hIsEqualTermNatSuccComp 
+          hIsEqualTermSigmaComp hIsEqualTermNatZeroComp hIsEqualTermNatSuccComp 
           hIsEqualTermIdenComp hIsEqualTermUnitIntroEq hIsEqualTermUnitElimEq hIsEqualTermEmptyElimEq
           hIsEqualTermPiIntroEq hIsEqualTermPiElimEq hIsEqualTermSigmaIntroEq
-          hIsEqualTermSigmaFirstEq hIsEqualTermSigmaSecondEq
+          hIsEqualTermSigmaElimEq
           hIsEqualTermNatZeroIntroEq hIsEqualTermNatSuccIntroEq
           hIsEqualTermNatElimEq
           hIsEqualTermIdenIntroEq hIsEqualTermIdenElimEq hIsEqualTermUnivUnitEq
@@ -386,7 +390,7 @@ theorem judgment_recursor :
           hHasTypeNatZeroIntro hHasTypeNatSuccIntro hHasTypeIdenIntro
           hHasTypeUnivUnit hHasTypeUnivEmpty hHasTypeUnivPi hHasTypeUnivSigma
           hHasTypeUnivNat hHasTypeUnivIden
-          hHasTypeUnitElim hHasTypeEmptyElim hHasTypePiElim hHasTypeSigmaFirst hHasTypeSigmaSecond 
+          hHasTypeUnitElim hHasTypeEmptyElim hHasTypePiElim hHasTypeSigmaElim
           hHasTypeNatElim hHasTypeIdenElim
           hHasTypeTyConv
         hIsEqualTypeUnitFormEq hIsEqualTypeEmptyFormEQ hIsEqualTypePiFormEq hIsEqualTypeSigmaFormEq
@@ -394,11 +398,10 @@ theorem judgment_recursor :
           hIsEqualTypeIdenFormEq hIsEqalTypeUnivFormEq hIsEqualTypeUnivElimEq
           hIsEqualTypeTypeSymm hIsEqualTypeTypeTrans
         hIsEqualTermVarEq hIsEqualTermWeakEq hIsEqualTermUnitComp hIsEqualTermPiComp
-          hIsEqualTermSigmaFirstComp hIsEqualTermSigmaSecondComp
-          hIsEqualTermNatZeroComp hIsEqualTermNatSuccComp 
+          hIsEqualTermSigmaComp hIsEqualTermNatZeroComp hIsEqualTermNatSuccComp 
           hIsEqualTermIdenComp hIsEqualTermUnitIntroEq hIsEqualTermUnitElimEq hIsEqualTermEmptyElimEq
           hIsEqualTermPiIntroEq hIsEqualTermPiElimEq hIsEqualTermSigmaIntroEq
-          hIsEqualTermSigmaFirstEq hIsEqualTermSigmaSecondEq
+          hIsEqualTermSigmaElimEq
           hIsEqualTermNatZeroIntroEq hIsEqualTermNatSuccIntroEq
           hIsEqualTermNatElimEq
           hIsEqualTermIdenIntroEq hIsEqualTermIdenElimEq hIsEqualTermUnivUnitEq
@@ -418,7 +421,7 @@ theorem judgment_recursor :
           hHasTypeNatZeroIntro hHasTypeNatSuccIntro hHasTypeIdenIntro
           hHasTypeUnivUnit hHasTypeUnivEmpty hHasTypeUnivPi hHasTypeUnivSigma
           hHasTypeUnivNat hHasTypeUnivIden
-          hHasTypeUnitElim hHasTypeEmptyElim hHasTypePiElim hHasTypeSigmaFirst hHasTypeSigmaSecond 
+          hHasTypeUnitElim hHasTypeEmptyElim hHasTypePiElim hHasTypeSigmaElim
           hHasTypeNatElim hHasTypeIdenElim
           hHasTypeTyConv
         hIsEqualTypeUnitFormEq hIsEqualTypeEmptyFormEQ hIsEqualTypePiFormEq hIsEqualTypeSigmaFormEq
@@ -426,11 +429,10 @@ theorem judgment_recursor :
           hIsEqualTypeIdenFormEq hIsEqalTypeUnivFormEq hIsEqualTypeUnivElimEq
           hIsEqualTypeTypeSymm hIsEqualTypeTypeTrans
         hIsEqualTermVarEq hIsEqualTermWeakEq hIsEqualTermUnitComp hIsEqualTermPiComp
-          hIsEqualTermSigmaFirstComp hIsEqualTermSigmaSecondComp
-          hIsEqualTermNatZeroComp hIsEqualTermNatSuccComp 
+          hIsEqualTermSigmaComp hIsEqualTermNatZeroComp hIsEqualTermNatSuccComp 
           hIsEqualTermIdenComp hIsEqualTermUnitIntroEq hIsEqualTermUnitElimEq hIsEqualTermEmptyElimEq
           hIsEqualTermPiIntroEq hIsEqualTermPiElimEq hIsEqualTermSigmaIntroEq
-          hIsEqualTermSigmaFirstEq hIsEqualTermSigmaSecondEq
+          hIsEqualTermSigmaElimEq
           hIsEqualTermNatZeroIntroEq hIsEqualTermNatSuccIntroEq
           hIsEqualTermNatElimEq
           hIsEqualTermIdenIntroEq hIsEqualTermIdenElimEq hIsEqualTermUnivUnitEq
@@ -450,7 +452,7 @@ theorem judgment_recursor :
           hHasTypeNatZeroIntro hHasTypeNatSuccIntro hHasTypeIdenIntro
           hHasTypeUnivUnit hHasTypeUnivEmpty hHasTypeUnivPi hHasTypeUnivSigma
           hHasTypeUnivNat hHasTypeUnivIden
-          hHasTypeUnitElim hHasTypeEmptyElim hHasTypePiElim hHasTypeSigmaFirst hHasTypeSigmaSecond 
+          hHasTypeUnitElim hHasTypeEmptyElim hHasTypePiElim hHasTypeSigmaElim
           hHasTypeNatElim hHasTypeIdenElim
           hHasTypeTyConv
         hIsEqualTypeUnitFormEq hIsEqualTypeEmptyFormEQ hIsEqualTypePiFormEq hIsEqualTypeSigmaFormEq
@@ -458,11 +460,10 @@ theorem judgment_recursor :
           hIsEqualTypeIdenFormEq hIsEqalTypeUnivFormEq hIsEqualTypeUnivElimEq
           hIsEqualTypeTypeSymm hIsEqualTypeTypeTrans
         hIsEqualTermVarEq hIsEqualTermWeakEq hIsEqualTermUnitComp hIsEqualTermPiComp
-          hIsEqualTermSigmaFirstComp hIsEqualTermSigmaSecondComp
-          hIsEqualTermNatZeroComp hIsEqualTermNatSuccComp 
+          hIsEqualTermSigmaComp hIsEqualTermNatZeroComp hIsEqualTermNatSuccComp 
           hIsEqualTermIdenComp hIsEqualTermUnitIntroEq hIsEqualTermUnitElimEq hIsEqualTermEmptyElimEq
           hIsEqualTermPiIntroEq hIsEqualTermPiElimEq hIsEqualTermSigmaIntroEq
-          hIsEqualTermSigmaFirstEq hIsEqualTermSigmaSecondEq
+          hIsEqualTermSigmaElimEq
           hIsEqualTermNatZeroIntroEq hIsEqualTermNatSuccIntroEq
           hIsEqualTermNatElimEq
           hIsEqualTermIdenIntroEq hIsEqualTermIdenElimEq hIsEqualTermUnivUnitEq
