IMLTT/typed/proofs/admissable/FunctionalityTyping/HasType.lean
@@ -1369,99 +1369,71 @@ theorem functionality_typing_pi_elim :
         · apply hsS'
         repeat' rfl
 
-theorem functionality_typing_sigma_first :
-    ∀ {n : Nat} {Γ : Ctx n} {p A : Tm n} {B : Tm (n + 1)},
-    (Γ ⊢ p ∶ ΣA;B) →
-    ((∀ (m l k : Nat) {leq : l ≤ m} (Γ_1 : Ctx l) (Δ : CtxGen (l + 1) (m + 1)) (Ξ : CtxGen (m + 2) (k + 1))
-          (eqM : n = k + 1) (s s' S : Tm l) (T : Tm (m + 1)),
-          (Γ_1 ⊢ s ≡ s' ∶ S) →
-            (Γ_1 ⊢ s ∶ S) →
-              (Γ_1 ⊢ s' ∶ S) →
-                eqM ▸ Γ = Γ_1 ⬝ S ⊗ Δ ⊙ T ⊗ Ξ → Γ_1 ⊗ ⌈s⌉(Δ w/Nat.le_refl l) ⊢ T⌈s/ₙleq⌉ ≡ T⌈s'/ₙleq⌉ type) ∧
-        ∀ (m l : Nat) {leq : l ≤ m} (Γ_1 : Ctx l) (Δ : CtxGen (l + 1) (m + 1)) (s s' S : Tm l) (t T : Tm (m + 1))
-          (eqM : n = m + 1),
-          (Γ_1 ⊢ s ≡ s' ∶ S) →
-            (Γ_1 ⊢ s ∶ S) →
-              (Γ_1 ⊢ s' ∶ S) →
-                eqM ▸ Γ = Γ_1 ⬝ S ⊗ Δ →
-                  eqM ▸ p = t → (eqM ▸ ΣA;B) = T → Γ_1 ⊗ ⌈s⌉(Δ w/Nat.le_refl l) ⊢ t⌈s/ₙleq⌉ ≡ t⌈s'/ₙleq⌉ ∶ T⌈s/ₙleq⌉) →
-      (∀ (m l k : Nat) {leq : l ≤ m} (Γ_1 : Ctx l) (Δ : CtxGen (l + 1) (m + 1)) (Ξ : CtxGen (m + 2) (k + 1))
-          (eqM : n = k + 1) (s s' S : Tm l) (T : Tm (m + 1)),
-          (Γ_1 ⊢ s ≡ s' ∶ S) →
-            (Γ_1 ⊢ s ∶ S) →
-              (Γ_1 ⊢ s' ∶ S) →
-                eqM ▸ Γ = Γ_1 ⬝ S ⊗ Δ ⊙ T ⊗ Ξ → Γ_1 ⊗ ⌈s⌉(Δ w/Nat.le_refl l) ⊢ T⌈s/ₙleq⌉ ≡ T⌈s'/ₙleq⌉ type) ∧
-        ∀ (m l : Nat) {leq : l ≤ m} (Γ_1 : Ctx l) (Δ : CtxGen (l + 1) (m + 1)) (s s' S : Tm l) (t T : Tm (m + 1))
-          (eqM : n = m + 1),
-          (Γ_1 ⊢ s ≡ s' ∶ S) →
-            (Γ_1 ⊢ s ∶ S) →
-              (Γ_1 ⊢ s' ∶ S) →
-                eqM ▸ Γ = Γ_1 ⬝ S ⊗ Δ →
-                  eqM ▸ π₁ p = t → eqM ▸ A = T → Γ_1 ⊗ ⌈s⌉(Δ w/Nat.le_refl l) ⊢ t⌈s/ₙleq⌉ ≡ t⌈s'/ₙleq⌉ ∶ T⌈s/ₙleq⌉ :=
+theorem functionality_typing_sigma_elim :
+  ∀ {n : Nat} {Γ : Ctx n} {A : Tm n} {B : Tm (n + 1)} {p : Tm n} {C : Tm (n + 1)} {c : Tm (n + 1 + 1)},
+  (Γ ⊢ p ∶ ΣA;B) →
+   (Γ ⬝ ΣA;B) ⊢ C type →
+     (Γ ⬝ A ⬝ B ⊢ c ∶ C⌈(ₛ↑ₚ↑ₚidₚ), v(1)&v(0)⌉) →
+       ((∀ (m l k : Nat) {leq : l ≤ m} (Γ_1 : Ctx l) (Δ : CtxGen (l + 1) (m + 1)) (Ξ : CtxGen (m + 2) (k + 1))
+             (eqM : n = k + 1) (s s' S : Tm l) (T : Tm (m + 1)),
+             (Γ_1 ⊢ s ≡ s' ∶ S) →
+               (Γ_1 ⊢ s ∶ S) →
+                 (Γ_1 ⊢ s' ∶ S) →
+                   eqM ▸ Γ = Γ_1 ⬝ S ⊗ Δ ⊙ T ⊗ Ξ → Γ_1 ⊗ ⌈s⌉(Δ w/Nat.le_refl l) ⊢ T⌈s/ₙleq⌉ ≡ T⌈s'/ₙleq⌉ type) ∧
+           ∀ (m l : Nat) {leq : l ≤ m} (Γ_1 : Ctx l) (Δ : CtxGen (l + 1) (m + 1)) (s s' S : Tm l) (t T : Tm (m + 1))
+             (eqM : n = m + 1),
+             (Γ_1 ⊢ s ≡ s' ∶ S) →
+               (Γ_1 ⊢ s ∶ S) →
+                 (Γ_1 ⊢ s' ∶ S) →
+                   eqM ▸ Γ = Γ_1 ⬝ S ⊗ Δ →
+                     eqM ▸ p = t →
+                       (eqM ▸ ΣA;B) = T → Γ_1 ⊗ ⌈s⌉(Δ w/Nat.le_refl l) ⊢ t⌈s/ₙleq⌉ ≡ t⌈s'/ₙleq⌉ ∶ T⌈s/ₙleq⌉) →
+         ((∀ (m l k : Nat) {leq : l ≤ m} (Γ_1 : Ctx l) (Δ : CtxGen (l + 1) (m + 1)) (Ξ : CtxGen (m + 2) (k + 1))
+               (eqM : n + 1 = k + 1) (s s' S : Tm l) (T : Tm (m + 1)),
+               (Γ_1 ⊢ s ≡ s' ∶ S) →
+                 (Γ_1 ⊢ s ∶ S) →
+                   (Γ_1 ⊢ s' ∶ S) →
+                     (eqM ▸ Γ ⬝ ΣA;B) = Γ_1 ⬝ S ⊗ Δ ⊙ T ⊗ Ξ →
+                       Γ_1 ⊗ ⌈s⌉(Δ w/Nat.le_refl l) ⊢ T⌈s/ₙleq⌉ ≡ T⌈s'/ₙleq⌉ type) ∧
+             ∀ (m l : Nat) {leq : l ≤ m} (Γ_1 : Ctx l) (Δ : CtxGen (l + 1) (m + 1)) (s s' S : Tm l) (T : Tm (m + 1))
+               (eqM : n + 1 = m + 1),
+               (Γ_1 ⊢ s ≡ s' ∶ S) →
+                 (Γ_1 ⊢ s ∶ S) →
+                   (Γ_1 ⊢ s' ∶ S) →
+                     (eqM ▸ Γ ⬝ ΣA;B) = Γ_1 ⬝ S ⊗ Δ →
+                       eqM ▸ C = T → Γ_1 ⊗ ⌈s⌉(Δ w/Nat.le_refl l) ⊢ T⌈s/ₙleq⌉ ≡ T⌈s'/ₙleq⌉ type) →
+           ((∀ (m l k : Nat) {leq : l ≤ m} (Γ_1 : Ctx l) (Δ : CtxGen (l + 1) (m + 1)) (Ξ : CtxGen (m + 2) (k + 1))
+                 (eqM : n + 1 + 1 = k + 1) (s s' S : Tm l) (T : Tm (m + 1)),
+                 (Γ_1 ⊢ s ≡ s' ∶ S) →
+                   (Γ_1 ⊢ s ∶ S) →
+                     (Γ_1 ⊢ s' ∶ S) →
+                       eqM ▸ Γ ⬝ A ⬝ B = Γ_1 ⬝ S ⊗ Δ ⊙ T ⊗ Ξ →
+                         Γ_1 ⊗ ⌈s⌉(Δ w/Nat.le_refl l) ⊢ T⌈s/ₙleq⌉ ≡ T⌈s'/ₙleq⌉ type) ∧
+               ∀ (m l : Nat) {leq : l ≤ m} (Γ_1 : Ctx l) (Δ : CtxGen (l + 1) (m + 1)) (s s' S : Tm l)
+                 (t T : Tm (m + 1)) (eqM : n + 1 + 1 = m + 1),
+                 (Γ_1 ⊢ s ≡ s' ∶ S) →
+                   (Γ_1 ⊢ s ∶ S) →
+                     (Γ_1 ⊢ s' ∶ S) →
+                       eqM ▸ Γ ⬝ A ⬝ B = Γ_1 ⬝ S ⊗ Δ →
+                         eqM ▸ c = t →
+                           eqM ▸ C⌈(ₛ↑ₚ↑ₚidₚ), v(1)&v(0)⌉ = T →
+                             Γ_1 ⊗ ⌈s⌉(Δ w/Nat.le_refl l) ⊢ t⌈s/ₙleq⌉ ≡ t⌈s'/ₙleq⌉ ∶ T⌈s/ₙleq⌉) →
+             (∀ (m l k : Nat) {leq : l ≤ m} (Γ_1 : Ctx l) (Δ : CtxGen (l + 1) (m + 1)) (Ξ : CtxGen (m + 2) (k + 1))
+                 (eqM : n = k + 1) (s s' S : Tm l) (T : Tm (m + 1)),
+                 (Γ_1 ⊢ s ≡ s' ∶ S) →
+                   (Γ_1 ⊢ s ∶ S) →
+                     (Γ_1 ⊢ s' ∶ S) →
+                       eqM ▸ Γ = Γ_1 ⬝ S ⊗ Δ ⊙ T ⊗ Ξ → Γ_1 ⊗ ⌈s⌉(Δ w/Nat.le_refl l) ⊢ T⌈s/ₙleq⌉ ≡ T⌈s'/ₙleq⌉ type) ∧
+               ∀ (m l : Nat) {leq : l ≤ m} (Γ_1 : Ctx l) (Δ : CtxGen (l + 1) (m + 1)) (s s' S : Tm l)
+                 (t T : Tm (m + 1)) (eqM : n = m + 1),
+                 (Γ_1 ⊢ s ≡ s' ∶ S) →
+                   (Γ_1 ⊢ s ∶ S) →
+                     (Γ_1 ⊢ s' ∶ S) →
+                       eqM ▸ Γ = Γ_1 ⬝ S ⊗ Δ →
+                         eqM ▸ A.indSigma B C c p = t →
+                           eqM ▸ C⌈p⌉₀ = T → Γ_1 ⊗ ⌈s⌉(Δ w/Nat.le_refl l) ⊢ t⌈s/ₙleq⌉ ≡ t⌈s'/ₙleq⌉ ∶ T⌈s/ₙleq⌉ :=
   by
-    intro n Γ' p A B hpSi ihpSi
-    apply And.intro
-    · intro m l k hleq Γ Δ Ξ heqM s s' S T hssS hsS hsS' heqΓ
-      cases heqM
-      cases heqΓ
-      apply And.left ihpSi
-      · apply hssS
-      · apply hsS
-      · apply hsS'
-      rotate_left
-      · apply k
-      · apply Ξ
-      · rfl
-      · rfl
-    · intro m l hleq Γ Δ s s' S t T heqM hssS hsS hsS' heqΓ heqt heqT
-      cases heqM
-      cases heqΓ
-      cases heqt
-      cases heqT
-      simp []
-      apply IsEqualTerm.sigma_first_eq
-      rotate_left
-      · apply B⌈1ₙ⇑ₛ(s/ₙhleq)⌉
-      · simp [lift_subst_n]
-        rw [←substitution_sigma]
-        apply And.right ihpSi
-        · apply hssS
-        · apply hsS
-        · apply hsS'
-        repeat' rfl
-
-theorem functionality_typing_sigma_second :
-    ∀ {n : Nat} {Γ : Ctx n} {p A : Tm n} {B : Tm (n + 1)},
-    (Γ ⊢ p ∶ ΣA;B) →
-    ((∀ (m l k : Nat) {leq : l ≤ m} (Γ_1 : Ctx l) (Δ : CtxGen (l + 1) (m + 1)) (Ξ : CtxGen (m + 2) (k + 1))
-          (eqM : n = k + 1) (s s' S : Tm l) (T : Tm (m + 1)),
-          (Γ_1 ⊢ s ≡ s' ∶ S) →
-            (Γ_1 ⊢ s ∶ S) →
-              (Γ_1 ⊢ s' ∶ S) →
-                eqM ▸ Γ = Γ_1 ⬝ S ⊗ Δ ⊙ T ⊗ Ξ → Γ_1 ⊗ ⌈s⌉(Δ w/Nat.le_refl l) ⊢ T⌈s/ₙleq⌉ ≡ T⌈s'/ₙleq⌉ type) ∧
-        ∀ (m l : Nat) {leq : l ≤ m} (Γ_1 : Ctx l) (Δ : CtxGen (l + 1) (m + 1)) (s s' S : Tm l) (t T : Tm (m + 1))
-          (eqM : n = m + 1),
-          (Γ_1 ⊢ s ≡ s' ∶ S) →
-            (Γ_1 ⊢ s ∶ S) →
-              (Γ_1 ⊢ s' ∶ S) →
-                eqM ▸ Γ = Γ_1 ⬝ S ⊗ Δ →
-                  eqM ▸ p = t → (eqM ▸ ΣA;B) = T → Γ_1 ⊗ ⌈s⌉(Δ w/Nat.le_refl l) ⊢ t⌈s/ₙleq⌉ ≡ t⌈s'/ₙleq⌉ ∶ T⌈s/ₙleq⌉) →
-      (∀ (m l k : Nat) {leq : l ≤ m} (Γ_1 : Ctx l) (Δ : CtxGen (l + 1) (m + 1)) (Ξ : CtxGen (m + 2) (k + 1))
-          (eqM : n = k + 1) (s s' S : Tm l) (T : Tm (m + 1)),
-          (Γ_1 ⊢ s ≡ s' ∶ S) →
-            (Γ_1 ⊢ s ∶ S) →
-              (Γ_1 ⊢ s' ∶ S) →
-                eqM ▸ Γ = Γ_1 ⬝ S ⊗ Δ ⊙ T ⊗ Ξ → Γ_1 ⊗ ⌈s⌉(Δ w/Nat.le_refl l) ⊢ T⌈s/ₙleq⌉ ≡ T⌈s'/ₙleq⌉ type) ∧
-        ∀ (m l : Nat) {leq : l ≤ m} (Γ_1 : Ctx l) (Δ : CtxGen (l + 1) (m + 1)) (s s' S : Tm l) (t T : Tm (m + 1))
-          (eqM : n = m + 1),
-          (Γ_1 ⊢ s ≡ s' ∶ S) →
-            (Γ_1 ⊢ s ∶ S) →
-              (Γ_1 ⊢ s' ∶ S) →
-                eqM ▸ Γ = Γ_1 ⬝ S ⊗ Δ →
-                  eqM ▸ π₂ p = t →
-                    eqM ▸ B⌈π₁ p⌉₀ = T → Γ_1 ⊗ ⌈s⌉(Δ w/Nat.le_refl l) ⊢ t⌈s/ₙleq⌉ ≡ t⌈s'/ₙleq⌉ ∶ T⌈s/ₙleq⌉ :=
-  by
-    intro n Γ' p A B hpSi ihpSi
+    intro n Γ' A B p C c hpSi hC hcC ihpSi ihC ihcC
     apply And.intro
     · intro m l k hleq Γ Δ Ξ heqM s s' S T hssS hsS hsS' heqΓ
       cases heqM
@@ -1481,11 +1453,51 @@ theorem functionality_typing_sigma_second :
       cases heqt
       cases heqT
       simp [substitution_zero_lift]
-      apply IsEqualTerm.sigma_second_eq
-      rotate_left
-      · apply A⌈(s/ₙhleq)⌉
-      · rw [←substitution_sigma]
+      apply IsEqualTerm.sigma_elim_eq
+      · apply And.left ihcC
+        · apply hssS
+        · apply hsS
+        · apply hsS'
+        rotate_left
+        · apply m + 1 + 1
+        · apply CtxGen.start ⊙ B
+        · rfl
+        · rfl
+      · simp [lift_subst_n]
+        simp [lift_n_substitution]
+        rw [extend_expand_context_n_substitution]
+        apply And.left ihcC
+        · apply hssS
+        · apply hsS
+        · apply hsS'
+        rotate_left
+        · apply m + 1 + 1
+        · apply CtxGen.start
+        · rfl
+        · rfl
+      · simp [lift_subst_n]
+        rw [←substitution_sigma]
         apply And.right ihpSi
+        · apply hssS
+        · apply hsS
+        · apply hsS'
+        repeat' rfl
+      · simp [lift_subst_n]
+        rw [←substitution_sigma]
+        rw [lift_n_substitution]
+        rw [lift_n_substitution]
+        rw [extend_expand_context_n_substitution]
+        apply And.right ihC
+        · apply hssS
+        · apply hsS
+        · apply hsS'
+        repeat' rfl
+      · simp [lift_subst_n]
+        rw [subst_subst_sigma_C]
+        simp [lift_n_substitution]
+        rw [extend_expand_context_n_substitution]
+        rw [extend_expand_context_n_substitution]
+        apply And.right ihcC
         · apply hssS
         · apply hsS
         · apply hsS'
