IMLTT/typed/proofs/admissable/WeakeningAlt/HasType.lean
@@ -10,287 +10,712 @@ import IMLTT.typed.JudgmentsAndRules
 import IMLTT.typed.proofs.Recursor
 import IMLTT.typed.proofs.boundary.BoundaryIsCtx
 
--- case HasTypeVar
--- ⊢ ∀ {x : Nat} {Γ : Ctx x} {A : Tm x},
---     Γ ⊢ A type →
---       (∀ (m l : Nat) (Γ_1 : Ctx l) (Δ : CtxGen l m) (eqM : x = m) (S : Tm l) (A_1 : Tm m),
---           Γ_1 ⊢ S type → eqM ▸ Γ = Γ_1 ⊗ Δ → eqM ▸ A = A_1 → (Γ_1 ⬝ S ⊗ ⌊↑₁↬l⌋Δ) ⊢ A_1⌊↑₁m↬l⌋ type) →
---         ∀ (m l : Nat) (Γ_1 : Ctx l) (Δ : CtxGen l m) (eqM : x + 1 = m) (S : Tm l) (a A_1 : Tm m),
---           Γ_1 ⊢ S type →
---             eqM ▸ Γ ⬝ A = Γ_1 ⊗ Δ → eqM ▸ v(0) = a → eqM ▸ A⌊↑ₚidₚ⌋ = A_1 → (Γ_1 ⬝ S ⊗ ⌊↑₁↬l⌋Δ) ⊢ a⌊↑₁m↬l⌋ ∶ A_1⌊↑₁m↬l⌋
--- case HasTypeWeak
--- ⊢ ∀ {x : Nat} {i : Fin x} {Γ : Ctx x} {A B : Tm x},
---     (Γ ⊢ v(i) ∶ A) →
---       Γ ⊢ B type →
---         (∀ (m l : Nat) (Γ_1 : Ctx l) (Δ : CtxGen l m) (eqM : x = m) (S : Tm l) (a A_1 : Tm m),
---             Γ_1 ⊢ S type →
---               eqM ▸ Γ = Γ_1 ⊗ Δ → eqM ▸ v(i) = a → eqM ▸ A = A_1 → (Γ_1 ⬝ S ⊗ ⌊↑₁↬l⌋Δ) ⊢ a⌊↑₁m↬l⌋ ∶ A_1⌊↑₁m↬l⌋) →
---           (∀ (m l : Nat) (Γ_1 : Ctx l) (Δ : CtxGen l m) (eqM : x = m) (S : Tm l) (A : Tm m),
---               Γ_1 ⊢ S type → eqM ▸ Γ = Γ_1 ⊗ Δ → eqM ▸ B = A → (Γ_1 ⬝ S ⊗ ⌊↑₁↬l⌋Δ) ⊢ A⌊↑₁m↬l⌋ type) →
---             ∀ (m l : Nat) (Γ_1 : Ctx l) (Δ : CtxGen l m) (eqM : x + 1 = m) (S : Tm l) (a A_1 : Tm m),
---               Γ_1 ⊢ S type →
---                 eqM ▸ Γ ⬝ B = Γ_1 ⊗ Δ →
---                   eqM ▸ v(i)⌊↑ₚidₚ⌋ = a → eqM ▸ A⌊↑ₚidₚ⌋ = A_1 → (Γ_1 ⬝ S ⊗ ⌊↑₁↬l⌋Δ) ⊢ a⌊↑₁m↬l⌋ ∶ A_1⌊↑₁m↬l⌋
--- case HasTypeUnitIntro
--- ⊢ ∀ {n : Nat} {Γ : Ctx n},
---     Γ ctx →
---       (∀ (m l : Nat) (Γ_1 : Ctx l) (Δ : CtxGen l m) (eqM : n = m) (S : Tm l),
---           Γ_1 ⊢ S type → eqM ▸ Γ = Γ_1 ⊗ Δ → (Γ_1 ⬝ S ⊗ ⌊↑₁↬l⌋Δ) ctx) →
---         ∀ (m l : Nat) (Γ_1 : Ctx l) (Δ : CtxGen l m) (eqM : n = m) (S : Tm l) (a A : Tm m),
---           Γ_1 ⊢ S type → eqM ▸ Γ = Γ_1 ⊗ Δ → eqM ▸ ⋆ = a → eqM ▸ 𝟙 = A → (Γ_1 ⬝ S ⊗ ⌊↑₁↬l⌋Δ) ⊢ a⌊↑₁m↬l⌋ ∶ A⌊↑₁m↬l⌋
--- case HasTypePiIntro
--- ⊢ ∀ {n : Nat} {Γ : Ctx n} {A : Tm n} {b B : Tm (n + 1)},
---     (Γ ⬝ A ⊢ b ∶ B) →
---       (∀ (m l : Nat) (Γ_1 : Ctx l) (Δ : CtxGen l m) (eqM : n + 1 = m) (S : Tm l) (a A_1 : Tm m),
---           Γ_1 ⊢ S type →
---             eqM ▸ Γ ⬝ A = Γ_1 ⊗ Δ → eqM ▸ b = a → eqM ▸ B = A_1 → (Γ_1 ⬝ S ⊗ ⌊↑₁↬l⌋Δ) ⊢ a⌊↑₁m↬l⌋ ∶ A_1⌊↑₁m↬l⌋) →
---         ∀ (m l : Nat) (Γ_1 : Ctx l) (Δ : CtxGen l m) (eqM : n = m) (S : Tm l) (a A_1 : Tm m),
---           Γ_1 ⊢ S type →
---             eqM ▸ Γ = Γ_1 ⊗ Δ → (eqM ▸ λA; b) = a → (eqM ▸ ΠA;B) = A_1 → (Γ_1 ⬝ S ⊗ ⌊↑₁↬l⌋Δ) ⊢ a⌊↑₁m↬l⌋ ∶ A_1⌊↑₁m↬l⌋
--- case HasTypeSigmaIntro
--- ⊢ ∀ {n : Nat} {Γ : Ctx n} {a A b : Tm n} {B : Tm (n + 1)},
---     (Γ ⊢ a ∶ A) →
---       (Γ ⊢ b ∶ B⌈a⌉₀) →
---         Γ ⬝ A ⊢ B type →
---           (∀ (m l : Nat) (Γ_1 : Ctx l) (Δ : CtxGen l m) (eqM : n = m) (S : Tm l) (a_4 A_1 : Tm m),
---               Γ_1 ⊢ S type →
---                 eqM ▸ Γ = Γ_1 ⊗ Δ → eqM ▸ a = a_4 → eqM ▸ A = A_1 → (Γ_1 ⬝ S ⊗ ⌊↑₁↬l⌋Δ) ⊢ a_4⌊↑₁m↬l⌋ ∶ A_1⌊↑₁m↬l⌋) →
---             (∀ (m l : Nat) (Γ_1 : Ctx l) (Δ : CtxGen l m) (eqM : n = m) (S : Tm l) (a_5 A : Tm m),
---                 Γ_1 ⊢ S type →
---                   eqM ▸ Γ = Γ_1 ⊗ Δ → eqM ▸ b = a_5 → eqM ▸ B⌈a⌉₀ = A → (Γ_1 ⬝ S ⊗ ⌊↑₁↬l⌋Δ) ⊢ a_5⌊↑₁m↬l⌋ ∶ A⌊↑₁m↬l⌋) →
---               (∀ (m l : Nat) (Γ_1 : Ctx l) (Δ : CtxGen l m) (eqM : n + 1 = m) (S : Tm l) (A_1 : Tm m),
---                   Γ_1 ⊢ S type → eqM ▸ Γ ⬝ A = Γ_1 ⊗ Δ → eqM ▸ B = A_1 → (Γ_1 ⬝ S ⊗ ⌊↑₁↬l⌋Δ) ⊢ A_1⌊↑₁m↬l⌋ type) →
---                 ∀ (m l : Nat) (Γ_1 : Ctx l) (Δ : CtxGen l m) (eqM : n = m) (S : Tm l) (a_7 A_1 : Tm m),
---                   Γ_1 ⊢ S type →
---                     eqM ▸ Γ = Γ_1 ⊗ Δ →
---                       eqM ▸ a&b = a_7 → (eqM ▸ ΣA;B) = A_1 → (Γ_1 ⬝ S ⊗ ⌊↑₁↬l⌋Δ) ⊢ a_7⌊↑₁m↬l⌋ ∶ A_1⌊↑₁m↬l⌋
--- case HasTypeNatZeroIntro
--- ⊢ ∀ {n : Nat} {Γ : Ctx n},
---     Γ ctx →
---       (∀ (m l : Nat) (Γ_1 : Ctx l) (Δ : CtxGen l m) (eqM : n = m) (S : Tm l),
---           Γ_1 ⊢ S type → eqM ▸ Γ = Γ_1 ⊗ Δ → (Γ_1 ⬝ S ⊗ ⌊↑₁↬l⌋Δ) ctx) →
---         ∀ (m l : Nat) (Γ_1 : Ctx l) (Δ : CtxGen l m) (eqM : n = m) (S : Tm l) (a A : Tm m),
---           Γ_1 ⊢ S type → eqM ▸ Γ = Γ_1 ⊗ Δ → eqM ▸ 𝓏 = a → eqM ▸ 𝒩 = A → (Γ_1 ⬝ S ⊗ ⌊↑₁↬l⌋Δ) ⊢ a⌊↑₁m↬l⌋ ∶ A⌊↑₁m↬l⌋
--- case HasTypeNatSuccIntro
--- ⊢ ∀ {n : Nat} {Γ : Ctx n} {x : Tm n},
---     (Γ ⊢ x ∶ 𝒩) →
---       (∀ (m l : Nat) (Γ_1 : Ctx l) (Δ : CtxGen l m) (eqM : n = m) (S : Tm l) (a A : Tm m),
---           Γ_1 ⊢ S type → eqM ▸ Γ = Γ_1 ⊗ Δ → eqM ▸ x = a → eqM ▸ 𝒩 = A → (Γ_1 ⬝ S ⊗ ⌊↑₁↬l⌋Δ) ⊢ a⌊↑₁m↬l⌋ ∶ A⌊↑₁m↬l⌋) →
---         ∀ (m l : Nat) (Γ_1 : Ctx l) (Δ : CtxGen l m) (eqM : n = m) (S : Tm l) (a A : Tm m),
---           Γ_1 ⊢ S type → eqM ▸ Γ = Γ_1 ⊗ Δ → eqM ▸ 𝓈(x) = a → eqM ▸ 𝒩 = A → (Γ_1 ⬝ S ⊗ ⌊↑₁↬l⌋Δ) ⊢ a⌊↑₁m↬l⌋ ∶ A⌊↑₁m↬l⌋
--- case HasTypeIdenIntro
--- ⊢ ∀ {n : Nat} {Γ : Ctx n} {A a : Tm n},
---     Γ ⊢ A type →
---       (Γ ⊢ a ∶ A) →
---         (∀ (m l : Nat) (Γ_1 : Ctx l) (Δ : CtxGen l m) (eqM : n = m) (S : Tm l) (A_1 : Tm m),
---             Γ_1 ⊢ S type → eqM ▸ Γ = Γ_1 ⊗ Δ → eqM ▸ A = A_1 → (Γ_1 ⬝ S ⊗ ⌊↑₁↬l⌋Δ) ⊢ A_1⌊↑₁m↬l⌋ type) →
---           (∀ (m l : Nat) (Γ_1 : Ctx l) (Δ : CtxGen l m) (eqM : n = m) (S : Tm l) (a_4 A_1 : Tm m),
---               Γ_1 ⊢ S type →
---                 eqM ▸ Γ = Γ_1 ⊗ Δ → eqM ▸ a = a_4 → eqM ▸ A = A_1 → (Γ_1 ⬝ S ⊗ ⌊↑₁↬l⌋Δ) ⊢ a_4⌊↑₁m↬l⌋ ∶ A_1⌊↑₁m↬l⌋) →
---             ∀ (m l : Nat) (Γ_1 : Ctx l) (Δ : CtxGen l m) (eqM : n = m) (S : Tm l) (a_5 A_1 : Tm m),
---               Γ_1 ⊢ S type →
---                 eqM ▸ Γ = Γ_1 ⊗ Δ →
---                   eqM ▸ A.refl a = a_5 → (eqM ▸ a ≃[A] a) = A_1 → (Γ_1 ⬝ S ⊗ ⌊↑₁↬l⌋Δ) ⊢ a_5⌊↑₁m↬l⌋ ∶ A_1⌊↑₁m↬l⌋
--- case HasTypeUnivUnit
--- ⊢ ∀ {n : Nat} {Γ : Ctx n},
---     Γ ctx →
---       (∀ (m l : Nat) (Γ_1 : Ctx l) (Δ : CtxGen l m) (eqM : n = m) (S : Tm l),
---           Γ_1 ⊢ S type → eqM ▸ Γ = Γ_1 ⊗ Δ → (Γ_1 ⬝ S ⊗ ⌊↑₁↬l⌋Δ) ctx) →
---         ∀ (m l : Nat) (Γ_1 : Ctx l) (Δ : CtxGen l m) (eqM : n = m) (S : Tm l) (a A : Tm m),
---           Γ_1 ⊢ S type → eqM ▸ Γ = Γ_1 ⊗ Δ → eqM ▸ 𝟙 = a → eqM ▸ 𝒰 = A → (Γ_1 ⬝ S ⊗ ⌊↑₁↬l⌋Δ) ⊢ a⌊↑₁m↬l⌋ ∶ A⌊↑₁m↬l⌋
--- case HasTypeUnivEmpty
--- ⊢ ∀ {n : Nat} {Γ : Ctx n},
---     Γ ctx →
---       (∀ (m l : Nat) (Γ_1 : Ctx l) (Δ : CtxGen l m) (eqM : n = m) (S : Tm l),
---           Γ_1 ⊢ S type → eqM ▸ Γ = Γ_1 ⊗ Δ → (Γ_1 ⬝ S ⊗ ⌊↑₁↬l⌋Δ) ctx) →
---         ∀ (m l : Nat) (Γ_1 : Ctx l) (Δ : CtxGen l m) (eqM : n = m) (S : Tm l) (a A : Tm m),
---           Γ_1 ⊢ S type → eqM ▸ Γ = Γ_1 ⊗ Δ → eqM ▸ 𝟘 = a → eqM ▸ 𝒰 = A → (Γ_1 ⬝ S ⊗ ⌊↑₁↬l⌋Δ) ⊢ a⌊↑₁m↬l⌋ ∶ A⌊↑₁m↬l⌋
--- case HasTypeUnivPi
--- ⊢ ∀ {n : Nat} {Γ : Ctx n} {A : Tm n} {B : Tm (n + 1)},
---     (Γ ⊢ A ∶ 𝒰) →
---       (Γ ⬝ A ⊢ B ∶ 𝒰) →
---         (∀ (m l : Nat) (Γ_1 : Ctx l) (Δ : CtxGen l m) (eqM : n = m) (S : Tm l) (a A_1 : Tm m),
---             Γ_1 ⊢ S type →
---               eqM ▸ Γ = Γ_1 ⊗ Δ → eqM ▸ A = a → eqM ▸ 𝒰 = A_1 → (Γ_1 ⬝ S ⊗ ⌊↑₁↬l⌋Δ) ⊢ a⌊↑₁m↬l⌋ ∶ A_1⌊↑₁m↬l⌋) →
---           (∀ (m l : Nat) (Γ_1 : Ctx l) (Δ : CtxGen l m) (eqM : n + 1 = m) (S : Tm l) (a A_1 : Tm m),
---               Γ_1 ⊢ S type →
---                 eqM ▸ Γ ⬝ A = Γ_1 ⊗ Δ → eqM ▸ B = a → eqM ▸ 𝒰 = A_1 → (Γ_1 ⬝ S ⊗ ⌊↑₁↬l⌋Δ) ⊢ a⌊↑₁m↬l⌋ ∶ A_1⌊↑₁m↬l⌋) →
---             ∀ (m l : Nat) (Γ_1 : Ctx l) (Δ : CtxGen l m) (eqM : n = m) (S : Tm l) (a A_1 : Tm m),
---               Γ_1 ⊢ S type →
---                 eqM ▸ Γ = Γ_1 ⊗ Δ → (eqM ▸ ΠA;B) = a → eqM ▸ 𝒰 = A_1 → (Γ_1 ⬝ S ⊗ ⌊↑₁↬l⌋Δ) ⊢ a⌊↑₁m↬l⌋ ∶ A_1⌊↑₁m↬l⌋
--- case HasTypeUnivSigma
--- ⊢ ∀ {n : Nat} {Γ : Ctx n} {A : Tm n} {B : Tm (n + 1)},
---     (Γ ⊢ A ∶ 𝒰) →
---       (Γ ⬝ A ⊢ B ∶ 𝒰) →
---         (∀ (m l : Nat) (Γ_1 : Ctx l) (Δ : CtxGen l m) (eqM : n = m) (S : Tm l) (a A_1 : Tm m),
---             Γ_1 ⊢ S type →
---               eqM ▸ Γ = Γ_1 ⊗ Δ → eqM ▸ A = a → eqM ▸ 𝒰 = A_1 → (Γ_1 ⬝ S ⊗ ⌊↑₁↬l⌋Δ) ⊢ a⌊↑₁m↬l⌋ ∶ A_1⌊↑₁m↬l⌋) →
---           (∀ (m l : Nat) (Γ_1 : Ctx l) (Δ : CtxGen l m) (eqM : n + 1 = m) (S : Tm l) (a A_1 : Tm m),
---               Γ_1 ⊢ S type →
---                 eqM ▸ Γ ⬝ A = Γ_1 ⊗ Δ → eqM ▸ B = a → eqM ▸ 𝒰 = A_1 → (Γ_1 ⬝ S ⊗ ⌊↑₁↬l⌋Δ) ⊢ a⌊↑₁m↬l⌋ ∶ A_1⌊↑₁m↬l⌋) →
---             ∀ (m l : Nat) (Γ_1 : Ctx l) (Δ : CtxGen l m) (eqM : n = m) (S : Tm l) (a A_1 : Tm m),
---               Γ_1 ⊢ S type →
---                 eqM ▸ Γ = Γ_1 ⊗ Δ → (eqM ▸ ΣA;B) = a → eqM ▸ 𝒰 = A_1 → (Γ_1 ⬝ S ⊗ ⌊↑₁↬l⌋Δ) ⊢ a⌊↑₁m↬l⌋ ∶ A_1⌊↑₁m↬l⌋
--- case HasTypeUnivNat
--- ⊢ ∀ {n : Nat} {Γ : Ctx n},
---     Γ ctx →
---       (∀ (m l : Nat) (Γ_1 : Ctx l) (Δ : CtxGen l m) (eqM : n = m) (S : Tm l),
---           Γ_1 ⊢ S type → eqM ▸ Γ = Γ_1 ⊗ Δ → (Γ_1 ⬝ S ⊗ ⌊↑₁↬l⌋Δ) ctx) →
---         ∀ (m l : Nat) (Γ_1 : Ctx l) (Δ : CtxGen l m) (eqM : n = m) (S : Tm l) (a A : Tm m),
---           Γ_1 ⊢ S type → eqM ▸ Γ = Γ_1 ⊗ Δ → eqM ▸ 𝒩 = a → eqM ▸ 𝒰 = A → (Γ_1 ⬝ S ⊗ ⌊↑₁↬l⌋Δ) ⊢ a⌊↑₁m↬l⌋ ∶ A⌊↑₁m↬l⌋
--- case HasTypeUnivIden
--- ⊢ ∀ {n : Nat} {Γ : Ctx n} {A a a' : Tm n},
---     (Γ ⊢ A ∶ 𝒰) →
---       (Γ ⊢ a ∶ A) →
---         (Γ ⊢ a' ∶ A) →
---           (∀ (m l : Nat) (Γ_1 : Ctx l) (Δ : CtxGen l m) (eqM : n = m) (S : Tm l) (a A_1 : Tm m),
---               Γ_1 ⊢ S type →
---                 eqM ▸ Γ = Γ_1 ⊗ Δ → eqM ▸ A = a → eqM ▸ 𝒰 = A_1 → (Γ_1 ⬝ S ⊗ ⌊↑₁↬l⌋Δ) ⊢ a⌊↑₁m↬l⌋ ∶ A_1⌊↑₁m↬l⌋) →
---             (∀ (m l : Nat) (Γ_1 : Ctx l) (Δ : CtxGen l m) (eqM : n = m) (S : Tm l) (a_5 A_1 : Tm m),
---                 Γ_1 ⊢ S type →
---                   eqM ▸ Γ = Γ_1 ⊗ Δ → eqM ▸ a = a_5 → eqM ▸ A = A_1 → (Γ_1 ⬝ S ⊗ ⌊↑₁↬l⌋Δ) ⊢ a_5⌊↑₁m↬l⌋ ∶ A_1⌊↑₁m↬l⌋) →
---               (∀ (m l : Nat) (Γ_1 : Ctx l) (Δ : CtxGen l m) (eqM : n = m) (S : Tm l) (a A_1 : Tm m),
---                   Γ_1 ⊢ S type →
---                     eqM ▸ Γ = Γ_1 ⊗ Δ → eqM ▸ a' = a → eqM ▸ A = A_1 → (Γ_1 ⬝ S ⊗ ⌊↑₁↬l⌋Δ) ⊢ a⌊↑₁m↬l⌋ ∶ A_1⌊↑₁m↬l⌋) →
---                 ∀ (m l : Nat) (Γ_1 : Ctx l) (Δ : CtxGen l m) (eqM : n = m) (S : Tm l) (a_7 A_1 : Tm m),
---                   Γ_1 ⊢ S type →
---                     eqM ▸ Γ = Γ_1 ⊗ Δ →
---                       (eqM ▸ a ≃[A] a') = a_7 → eqM ▸ 𝒰 = A_1 → (Γ_1 ⬝ S ⊗ ⌊↑₁↬l⌋Δ) ⊢ a_7⌊↑₁m↬l⌋ ∶ A_1⌊↑₁m↬l⌋
--- case HasTypeUnitElim
--- ⊢ ∀ {n : Nat} {Γ : Ctx n} {A : Tm (n + 1)} {a b : Tm n},
---     Γ ⬝ 𝟙 ⊢ A type →
---       (Γ ⊢ a ∶ A⌈⋆⌉₀) →
---         (Γ ⊢ b ∶ 𝟙) →
---           (∀ (m l : Nat) (Γ_1 : Ctx l) (Δ : CtxGen l m) (eqM : n + 1 = m) (S : Tm l) (A_1 : Tm m),
---               Γ_1 ⊢ S type → eqM ▸ Γ ⬝ 𝟙 = Γ_1 ⊗ Δ → eqM ▸ A = A_1 → (Γ_1 ⬝ S ⊗ ⌊↑₁↬l⌋Δ) ⊢ A_1⌊↑₁m↬l⌋ type) →
---             (∀ (m l : Nat) (Γ_1 : Ctx l) (Δ : CtxGen l m) (eqM : n = m) (S : Tm l) (a_5 A_1 : Tm m),
---                 Γ_1 ⊢ S type →
---                   eqM ▸ Γ = Γ_1 ⊗ Δ → eqM ▸ a = a_5 → eqM ▸ A⌈⋆⌉₀ = A_1 → (Γ_1 ⬝ S ⊗ ⌊↑₁↬l⌋Δ) ⊢ a_5⌊↑₁m↬l⌋ ∶ A_1⌊↑₁m↬l⌋) →
---               (∀ (m l : Nat) (Γ_1 : Ctx l) (Δ : CtxGen l m) (eqM : n = m) (S : Tm l) (a A : Tm m),
---                   Γ_1 ⊢ S type →
---                     eqM ▸ Γ = Γ_1 ⊗ Δ → eqM ▸ b = a → eqM ▸ 𝟙 = A → (Γ_1 ⬝ S ⊗ ⌊↑₁↬l⌋Δ) ⊢ a⌊↑₁m↬l⌋ ∶ A⌊↑₁m↬l⌋) →
---                 ∀ (m l : Nat) (Γ_1 : Ctx l) (Δ : CtxGen l m) (eqM : n = m) (S : Tm l) (a_7 A_1 : Tm m),
---                   Γ_1 ⊢ S type →
---                     eqM ▸ Γ = Γ_1 ⊗ Δ →
---                       eqM ▸ A.indUnit b a = a_7 → eqM ▸ A⌈b⌉₀ = A_1 → (Γ_1 ⬝ S ⊗ ⌊↑₁↬l⌋Δ) ⊢ a_7⌊↑₁m↬l⌋ ∶ A_1⌊↑₁m↬l⌋
--- case HasTypeEmptyElim
--- ⊢ ∀ {n : Nat} {Γ : Ctx n} {A : Tm (n + 1)} {b : Tm n},
---     Γ ⬝ 𝟘 ⊢ A type →
---       (Γ ⊢ b ∶ 𝟘) →
---         (∀ (m l : Nat) (Γ_1 : Ctx l) (Δ : CtxGen l m) (eqM : n + 1 = m) (S : Tm l) (A_1 : Tm m),
---             Γ_1 ⊢ S type → eqM ▸ Γ ⬝ 𝟘 = Γ_1 ⊗ Δ → eqM ▸ A = A_1 → (Γ_1 ⬝ S ⊗ ⌊↑₁↬l⌋Δ) ⊢ A_1⌊↑₁m↬l⌋ type) →
---           (∀ (m l : Nat) (Γ_1 : Ctx l) (Δ : CtxGen l m) (eqM : n = m) (S : Tm l) (a A : Tm m),
---               Γ_1 ⊢ S type → eqM ▸ Γ = Γ_1 ⊗ Δ → eqM ▸ b = a → eqM ▸ 𝟘 = A → (Γ_1 ⬝ S ⊗ ⌊↑₁↬l⌋Δ) ⊢ a⌊↑₁m↬l⌋ ∶ A⌊↑₁m↬l⌋) →
---             ∀ (m l : Nat) (Γ_1 : Ctx l) (Δ : CtxGen l m) (eqM : n = m) (S : Tm l) (a A_1 : Tm m),
---               Γ_1 ⊢ S type →
---                 eqM ▸ Γ = Γ_1 ⊗ Δ →
---                   eqM ▸ A.indEmpty b = a → eqM ▸ A⌈b⌉₀ = A_1 → (Γ_1 ⬝ S ⊗ ⌊↑₁↬l⌋Δ) ⊢ a⌊↑₁m↬l⌋ ∶ A_1⌊↑₁m↬l⌋
--- case HasTypePiElim
--- ⊢ ∀ {n : Nat} {Γ : Ctx n} {f A : Tm n} {B : Tm (n + 1)} {a : Tm n},
---     (Γ ⊢ f ∶ ΠA;B) →
---       (Γ ⊢ a ∶ A) →
---         (∀ (m l : Nat) (Γ_1 : Ctx l) (Δ : CtxGen l m) (eqM : n = m) (S : Tm l) (a A_1 : Tm m),
---             Γ_1 ⊢ S type →
---               eqM ▸ Γ = Γ_1 ⊗ Δ → eqM ▸ f = a → (eqM ▸ ΠA;B) = A_1 → (Γ_1 ⬝ S ⊗ ⌊↑₁↬l⌋Δ) ⊢ a⌊↑₁m↬l⌋ ∶ A_1⌊↑₁m↬l⌋) →
---           (∀ (m l : Nat) (Γ_1 : Ctx l) (Δ : CtxGen l m) (eqM : n = m) (S : Tm l) (a_4 A_1 : Tm m),
---               Γ_1 ⊢ S type →
---                 eqM ▸ Γ = Γ_1 ⊗ Δ → eqM ▸ a = a_4 → eqM ▸ A = A_1 → (Γ_1 ⬝ S ⊗ ⌊↑₁↬l⌋Δ) ⊢ a_4⌊↑₁m↬l⌋ ∶ A_1⌊↑₁m↬l⌋) →
---             ∀ (m l : Nat) (Γ_1 : Ctx l) (Δ : CtxGen l m) (eqM : n = m) (S : Tm l) (a_5 A : Tm m),
---               Γ_1 ⊢ S type →
---                 eqM ▸ Γ = Γ_1 ⊗ Δ → eqM ▸ f◃a = a_5 → eqM ▸ B⌈a⌉₀ = A → (Γ_1 ⬝ S ⊗ ⌊↑₁↬l⌋Δ) ⊢ a_5⌊↑₁m↬l⌋ ∶ A⌊↑₁m↬l⌋
--- case HasTypeSigmaFirst
--- ⊢ ∀ {n : Nat} {Γ : Ctx n} {p A : Tm n} {B : Tm (n + 1)},
---     (Γ ⊢ p ∶ ΣA;B) →
---       (∀ (m l : Nat) (Γ_1 : Ctx l) (Δ : CtxGen l m) (eqM : n = m) (S : Tm l) (a A_1 : Tm m),
---           Γ_1 ⊢ S type →
---             eqM ▸ Γ = Γ_1 ⊗ Δ → eqM ▸ p = a → (eqM ▸ ΣA;B) = A_1 → (Γ_1 ⬝ S ⊗ ⌊↑₁↬l⌋Δ) ⊢ a⌊↑₁m↬l⌋ ∶ A_1⌊↑₁m↬l⌋) →
---         ∀ (m l : Nat) (Γ_1 : Ctx l) (Δ : CtxGen l m) (eqM : n = m) (S : Tm l) (a A_1 : Tm m),
---           Γ_1 ⊢ S type → eqM ▸ Γ = Γ_1 ⊗ Δ → eqM ▸ π₁ p = a → eqM ▸ A = A_1 → (Γ_1 ⬝ S ⊗ ⌊↑₁↬l⌋Δ) ⊢ a⌊↑₁m↬l⌋ ∶ A_1⌊↑₁m↬l⌋
--- case HasTypeSigmaSecond
--- ⊢ ∀ {n : Nat} {Γ : Ctx n} {p A : Tm n} {B : Tm (n + 1)},
---     (Γ ⊢ p ∶ ΣA;B) →
---       (∀ (m l : Nat) (Γ_1 : Ctx l) (Δ : CtxGen l m) (eqM : n = m) (S : Tm l) (a A_1 : Tm m),
---           Γ_1 ⊢ S type →
---             eqM ▸ Γ = Γ_1 ⊗ Δ → eqM ▸ p = a → (eqM ▸ ΣA;B) = A_1 → (Γ_1 ⬝ S ⊗ ⌊↑₁↬l⌋Δ) ⊢ a⌊↑₁m↬l⌋ ∶ A_1⌊↑₁m↬l⌋) →
---         ∀ (m l : Nat) (Γ_1 : Ctx l) (Δ : CtxGen l m) (eqM : n = m) (S : Tm l) (a A : Tm m),
---           Γ_1 ⊢ S type →
---             eqM ▸ Γ = Γ_1 ⊗ Δ → eqM ▸ π₂ p = a → eqM ▸ B⌈π₁ p⌉₀ = A → (Γ_1 ⬝ S ⊗ ⌊↑₁↬l⌋Δ) ⊢ a⌊↑₁m↬l⌋ ∶ A⌊↑₁m↬l⌋
--- case HasTypeNatElim
--- ⊢ ∀ {n : Nat} {Γ : Ctx n} {z x : Tm n} {A : Tm (n + 1)} {s : Tm (n + 2)},
---     Γ ⬝ 𝒩 ⊢ A type →
---       (Γ ⊢ z ∶ A⌈𝓏⌉₀) →
---         (Γ ⬝ 𝒩 ⬝ A ⊢ s ∶ A⌈(ₛ↑ₚidₚ), 𝓈(v(0))⌉⌊↑ₚidₚ⌋) →
---           (Γ ⊢ x ∶ 𝒩) →
---             (∀ (m l : Nat) (Γ_1 : Ctx l) (Δ : CtxGen l m) (eqM : n + 1 = m) (S : Tm l) (A_1 : Tm m),
---                 Γ_1 ⊢ S type → eqM ▸ Γ ⬝ 𝒩 = Γ_1 ⊗ Δ → eqM ▸ A = A_1 → (Γ_1 ⬝ S ⊗ ⌊↑₁↬l⌋Δ) ⊢ A_1⌊↑₁m↬l⌋ type) →
---               (∀ (m l : Nat) (Γ_1 : Ctx l) (Δ : CtxGen l m) (eqM : n = m) (S : Tm l) (a A_1 : Tm m),
---                   Γ_1 ⊢ S type →
---                     eqM ▸ Γ = Γ_1 ⊗ Δ → eqM ▸ z = a → eqM ▸ A⌈𝓏⌉₀ = A_1 → (Γ_1 ⬝ S ⊗ ⌊↑₁↬l⌋Δ) ⊢ a⌊↑₁m↬l⌋ ∶ A_1⌊↑₁m↬l⌋) →
---                 (∀ (m l : Nat) (Γ_1 : Ctx l) (Δ : CtxGen l m) (eqM : n + 1 + 1 = m) (S : Tm l) (a A_1 : Tm m),
---                     Γ_1 ⊢ S type →
---                       eqM ▸ Γ ⬝ 𝒩 ⬝ A = Γ_1 ⊗ Δ →
---                         eqM ▸ s = a →
---                           eqM ▸ A⌈(ₛ↑ₚidₚ), 𝓈(v(0))⌉⌊↑ₚidₚ⌋ = A_1 → (Γ_1 ⬝ S ⊗ ⌊↑₁↬l⌋Δ) ⊢ a⌊↑₁m↬l⌋ ∶ A_1⌊↑₁m↬l⌋) →
---                   (∀ (m l : Nat) (Γ_1 : Ctx l) (Δ : CtxGen l m) (eqM : n = m) (S : Tm l) (a A : Tm m),
---                       Γ_1 ⊢ S type →
---                         eqM ▸ Γ = Γ_1 ⊗ Δ → eqM ▸ x = a → eqM ▸ 𝒩 = A → (Γ_1 ⬝ S ⊗ ⌊↑₁↬l⌋Δ) ⊢ a⌊↑₁m↬l⌋ ∶ A⌊↑₁m↬l⌋) →
---                     ∀ (m l : Nat) (Γ_1 : Ctx l) (Δ : CtxGen l m) (eqM : n = m) (S : Tm l) (a A_1 : Tm m),
---                       Γ_1 ⊢ S type →
---                         eqM ▸ Γ = Γ_1 ⊗ Δ →
---                           eqM ▸ A.indNat z s x = a → eqM ▸ A⌈x⌉₀ = A_1 → (Γ_1 ⬝ S ⊗ ⌊↑₁↬l⌋Δ) ⊢ a⌊↑₁m↬l⌋ ∶ A_1⌊↑₁m↬l⌋
--- case HasTypeIdenElim
--- ⊢ ∀ {n : Nat} {Γ : Ctx n} {A : Tm n} {B : Tm (n + 1 + 1 + 1)} {b a a' p : Tm n},
---     (Γ ⬝ A ⬝ A⌊↑ₚidₚ⌋ ⬝ v(1) ≃[A⌊↑ₚ↑ₚidₚ⌋] v(0)) ⊢ B type →
---       (Γ ⊢ b ∶ B⌈(ₛidₚ), a, a, A.refl a⌉) →
---         (Γ ⊢ a ∶ A) →
---           (Γ ⊢ a' ∶ A) →
---             (Γ ⊢ p ∶ a ≃[A] a') →
---               Γ ⊢ B⌈(ₛidₚ), a, a, A.refl a⌉ type →
---                 Γ ⊢ B⌈(ₛidₚ), a, a', p⌉ type →
---                   (∀ (m l : Nat) (Γ_1 : Ctx l) (Δ : CtxGen l m) (eqM : n + 1 + 1 + 1 = m) (S : Tm l) (A_1 : Tm m),
---                       Γ_1 ⊢ S type →
---                         (eqM ▸ Γ ⬝ A ⬝ A⌊↑ₚidₚ⌋ ⬝ v(1) ≃[A⌊↑ₚ↑ₚidₚ⌋] v(0)) = Γ_1 ⊗ Δ →
---                           eqM ▸ B = A_1 → (Γ_1 ⬝ S ⊗ ⌊↑₁↬l⌋Δ) ⊢ A_1⌊↑₁m↬l⌋ type) →
---                     (∀ (m l : Nat) (Γ_1 : Ctx l) (Δ : CtxGen l m) (eqM : n = m) (S : Tm l) (a_7 A_1 : Tm m),
---                         Γ_1 ⊢ S type →
---                           eqM ▸ Γ = Γ_1 ⊗ Δ →
---                             eqM ▸ b = a_7 →
---                               eqM ▸ B⌈(ₛidₚ), a, a, A.refl a⌉ = A_1 → (Γ_1 ⬝ S ⊗ ⌊↑₁↬l⌋Δ) ⊢ a_7⌊↑₁m↬l⌋ ∶ A_1⌊↑₁m↬l⌋) →
---                       (∀ (m l : Nat) (Γ_1 : Ctx l) (Δ : CtxGen l m) (eqM : n = m) (S : Tm l) (a_8 A_1 : Tm m),
---                           Γ_1 ⊢ S type →
---                             eqM ▸ Γ = Γ_1 ⊗ Δ →
---                               eqM ▸ a = a_8 → eqM ▸ A = A_1 → (Γ_1 ⬝ S ⊗ ⌊↑₁↬l⌋Δ) ⊢ a_8⌊↑₁m↬l⌋ ∶ A_1⌊↑₁m↬l⌋) →
---                         (∀ (m l : Nat) (Γ_1 : Ctx l) (Δ : CtxGen l m) (eqM : n = m) (S : Tm l) (a A_1 : Tm m),
---                             Γ_1 ⊢ S type →
---                               eqM ▸ Γ = Γ_1 ⊗ Δ →
---                                 eqM ▸ a' = a → eqM ▸ A = A_1 → (Γ_1 ⬝ S ⊗ ⌊↑₁↬l⌋Δ) ⊢ a⌊↑₁m↬l⌋ ∶ A_1⌊↑₁m↬l⌋) →
---                           (∀ (m l : Nat) (Γ_1 : Ctx l) (Δ : CtxGen l m) (eqM : n = m) (S : Tm l) (a_10 A_1 : Tm m),
---                               Γ_1 ⊢ S type →
---                                 eqM ▸ Γ = Γ_1 ⊗ Δ →
---                                   eqM ▸ p = a_10 →
---                                     (eqM ▸ a ≃[A] a') = A_1 → (Γ_1 ⬝ S ⊗ ⌊↑₁↬l⌋Δ) ⊢ a_10⌊↑₁m↬l⌋ ∶ A_1⌊↑₁m↬l⌋) →
---                             (∀ (m l : Nat) (Γ_1 : Ctx l) (Δ : CtxGen l m) (eqM : n = m) (S : Tm l) (A_1 : Tm m),
---                                 Γ_1 ⊢ S type →
---                                   eqM ▸ Γ = Γ_1 ⊗ Δ →
---                                     eqM ▸ B⌈(ₛidₚ), a, a, A.refl a⌉ = A_1 → (Γ_1 ⬝ S ⊗ ⌊↑₁↬l⌋Δ) ⊢ A_1⌊↑₁m↬l⌋ type) →
---                               (∀ (m l : Nat) (Γ_1 : Ctx l) (Δ : CtxGen l m) (eqM : n = m) (S : Tm l) (A : Tm m),
---                                   Γ_1 ⊢ S type →
---                                     eqM ▸ Γ = Γ_1 ⊗ Δ →
---                                       eqM ▸ B⌈(ₛidₚ), a, a', p⌉ = A → (Γ_1 ⬝ S ⊗ ⌊↑₁↬l⌋Δ) ⊢ A⌊↑₁m↬l⌋ type) →
---                                 ∀ (m l : Nat) (Γ_1 : Ctx l) (Δ : CtxGen l m) (eqM : n = m) (S : Tm l) (a_13 A_1 : Tm m),
---                                   Γ_1 ⊢ S type →
---                                     eqM ▸ Γ = Γ_1 ⊗ Δ →
---                                       eqM ▸ A.j B b a a' p = a_13 →
---                                         eqM ▸ B⌈(ₛidₚ), a, a', p⌉ = A_1 → (Γ_1 ⬝ S ⊗ ⌊↑₁↬l⌋Δ) ⊢ a_13⌊↑₁m↬l⌋ ∶ A_1⌊↑₁m↬l⌋
--- case HasTypeTyConv
--- ⊢ ∀ {n : Nat} {Γ : Ctx n} {a A B : Tm n},
---     (Γ ⊢ a ∶ A) →
---       Γ ⊢ A ≡ B type →
---         (∀ (m l : Nat) (Γ_1 : Ctx l) (Δ : CtxGen l m) (eqM : n = m) (S : Tm l) (a_3 A_1 : Tm m),
---             Γ_1 ⊢ S type →
---               eqM ▸ Γ = Γ_1 ⊗ Δ → eqM ▸ a = a_3 → eqM ▸ A = A_1 → (Γ_1 ⬝ S ⊗ ⌊↑₁↬l⌋Δ) ⊢ a_3⌊↑₁m↬l⌋ ∶ A_1⌊↑₁m↬l⌋) →
---           (∀ (m l : Nat) (Γ_1 : Ctx l) (Δ : CtxGen l m) (eqM : n = m) (S : Tm l) (A_1 A' : Tm m),
---               Γ_1 ⊢ S type →
---                 eqM ▸ Γ = Γ_1 ⊗ Δ → eqM ▸ A = A_1 → eqM ▸ B = A' → (Γ_1 ⬝ S ⊗ ⌊↑₁↬l⌋Δ) ⊢ A_1⌊↑₁m↬l⌋ ≡ A'⌊↑₁m↬l⌋ type) →
---             ∀ (m l : Nat) (Γ_1 : Ctx l) (Δ : CtxGen l m) (eqM : n = m) (S : Tm l) (a_5 A : Tm m),
---               Γ_1 ⊢ S type → eqM ▸ Γ = Γ_1 ⊗ Δ → eqM ▸ a = a_5 → eqM ▸ B = A → (Γ_1 ⬝ S ⊗ ⌊↑₁↬l⌋Δ) ⊢ a_5⌊↑₁m↬l⌋ ∶ A⌊↑₁m↬l⌋
+import IMLTT.typed.proofs.admissable.weakening.Helpers
+
+theorem weakening_var :
+    ∀ {x : Nat} {Γ : Ctx x} {A : Tm x},
+      Γ ⊢ A type →
+        (∀ (m l : Nat) (Γ_1 : Ctx l) (Δ : CtxGen l m) (eqM : x = m) (S : Tm l) (A_1 : Tm m),
+            Γ_1 ⊢ S type → eqM ▸ Γ = Γ_1 ⊗ Δ → eqM ▸ A = A_1 → (Γ_1 ⬝ S ⊗ ⌊↑₁↬l⌋Δ) ⊢ A_1⌊↑₁m↬l⌋ type) →
+          ∀ (m l : Nat) (Γ_1 : Ctx l) (Δ : CtxGen l m) (eqM : x + 1 = m) (S : Tm l) (a A_1 : Tm m),
+            Γ_1 ⊢ S type →
+              eqM ▸ Γ ⬝ A = Γ_1 ⊗ Δ → eqM ▸ v(0) = a → eqM ▸ A⌊↑ₚidₚ⌋ = A_1 → (Γ_1 ⬝ S ⊗ ⌊↑₁↬l⌋Δ) ⊢ a⌊↑₁m↬l⌋ ∶ A_1⌊↑₁m↬l⌋ :=
+  by
+    intro n Γ A hA ihA m l Γ Δ heqM S t T hS heqΓ heqt heqT
+    cases heqM
+    cases heqt
+    cases heqT
+    cases Δ with
+    | start =>
+      cases heqΓ
+      simp [empty_expand_context_weaken_from]
+      simp [expand_ctx]
+      simp [weaken_from_zero]
+      apply HasType.weak
+      · apply HasType.var
+        apply ctx_extr (boundary_ctx_type hS)
+      · apply hS
+    | expand Δ' S' =>
+      cases heqΓ
+      rw [←extend_expand_context_weaken_from]
+      rw [shift_weaken_from]
+      rw [←lift_weaken_from]
+      rw [weaken]
+      simp [weaken_var]
+      apply HasType.var
+      apply ihA
+      apply hS
+      repeat' rfl
+      any_goals apply gen_ctx_leq Δ'
+
+theorem weakening_weak :
+    ∀ {x : Nat} {i : Fin x} {Γ : Ctx x} {A B : Tm x},
+      (Γ ⊢ v(i) ∶ A) →
+        Γ ⊢ B type →
+          (∀ (m l : Nat) (Γ_1 : Ctx l) (Δ : CtxGen l m) (eqM : x = m) (S : Tm l) (a A_1 : Tm m),
+              Γ_1 ⊢ S type →
+                eqM ▸ Γ = Γ_1 ⊗ Δ → eqM ▸ v(i) = a → eqM ▸ A = A_1 → (Γ_1 ⬝ S ⊗ ⌊↑₁↬l⌋Δ) ⊢ a⌊↑₁m↬l⌋ ∶ A_1⌊↑₁m↬l⌋) →
+            (∀ (m l : Nat) (Γ_1 : Ctx l) (Δ : CtxGen l m) (eqM : x = m) (S : Tm l) (A : Tm m),
+                Γ_1 ⊢ S type → eqM ▸ Γ = Γ_1 ⊗ Δ → eqM ▸ B = A → (Γ_1 ⬝ S ⊗ ⌊↑₁↬l⌋Δ) ⊢ A⌊↑₁m↬l⌋ type) →
+              ∀ (m l : Nat) (Γ_1 : Ctx l) (Δ : CtxGen l m) (eqM : x + 1 = m) (S : Tm l) (a A_1 : Tm m),
+                Γ_1 ⊢ S type →
+                  eqM ▸ Γ ⬝ B = Γ_1 ⊗ Δ →
+                    eqM ▸ v(i)⌊↑ₚidₚ⌋ = a → eqM ▸ A⌊↑ₚidₚ⌋ = A_1 → (Γ_1 ⬝ S ⊗ ⌊↑₁↬l⌋Δ) ⊢ a⌊↑₁m↬l⌋ ∶ A_1⌊↑₁m↬l⌋ :=
+  by
+    intro n x Γ A B hvA hB ihvA ihB m l Γ Δ heqM S t T hS heqΓ heqt heqT
+    cases heqM
+    cases heqt
+    cases heqT
+    cases Δ with
+    | start =>
+      cases heqΓ
+      simp [empty_expand_context_weaken_from]
+      simp [expand_ctx]
+      simp [weaken_from_zero]
+      apply HasType.weak
+      · simp [←weakening_conv_var]
+        apply HasType.weak
+        · apply hvA
+        · apply ctx_extr (boundary_ctx_type hS)
+      · apply hS
+    | expand Δ' S' =>
+      cases heqΓ
+      rw [←extend_expand_context_weaken_from]
+      rw [shift_weaken_from]
+      rw [shift_weaken_from]
+      apply HasType.weak
+      · rw [←weakening_conv_var]
+        apply ihvA
+        apply hS
+        repeat' rfl
+      · apply ihB
+        apply hS
+        repeat' rfl
+      any_goals apply gen_ctx_leq Δ'
+
+theorem weakening_unit_intro :
+    ∀ {n : Nat} {Γ : Ctx n},
+      Γ ctx →
+        (∀ (m l : Nat) (Γ_1 : Ctx l) (Δ : CtxGen l m) (eqM : n = m) (S : Tm l),
+            Γ_1 ⊢ S type → eqM ▸ Γ = Γ_1 ⊗ Δ → (Γ_1 ⬝ S ⊗ ⌊↑₁↬l⌋Δ) ctx) →
+          ∀ (m l : Nat) (Γ_1 : Ctx l) (Δ : CtxGen l m) (eqM : n = m) (S : Tm l) (a A : Tm m),
+            Γ_1 ⊢ S type → eqM ▸ Γ = Γ_1 ⊗ Δ → eqM ▸ ⋆ = a → eqM ▸ 𝟙 = A → (Γ_1 ⬝ S ⊗ ⌊↑₁↬l⌋Δ) ⊢ a⌊↑₁m↬l⌋ ∶ A⌊↑₁m↬l⌋ :=
+  by
+    intro n Γ' hiC ihiC m l Γ Δ heqM S t T hS heqΓ heqt heqT
+    cases heqM
+    cases heqΓ
+    cases heqt
+    cases heqT
+    apply HasType.unit_intro
+    apply ihiC
+    apply hS
+    repeat' rfl
+
+theorem weakening_pi_intro :
+    ∀ {n : Nat} {Γ : Ctx n} {A : Tm n} {b B : Tm (n + 1)},
+      (Γ ⬝ A ⊢ b ∶ B) →
+        (∀ (m l : Nat) (Γ_1 : Ctx l) (Δ : CtxGen l m) (eqM : n + 1 = m) (S : Tm l) (a A_1 : Tm m),
+            Γ_1 ⊢ S type →
+              eqM ▸ Γ ⬝ A = Γ_1 ⊗ Δ → eqM ▸ b = a → eqM ▸ B = A_1 → (Γ_1 ⬝ S ⊗ ⌊↑₁↬l⌋Δ) ⊢ a⌊↑₁m↬l⌋ ∶ A_1⌊↑₁m↬l⌋) →
+          ∀ (m l : Nat) (Γ_1 : Ctx l) (Δ : CtxGen l m) (eqM : n = m) (S : Tm l) (a A_1 : Tm m),
+            Γ_1 ⊢ S type →
+              eqM ▸ Γ = Γ_1 ⊗ Δ → (eqM ▸ λA; b) = a → (eqM ▸ ΠA;B) = A_1 → (Γ_1 ⬝ S ⊗ ⌊↑₁↬l⌋Δ) ⊢ a⌊↑₁m↬l⌋ ∶ A_1⌊↑₁m↬l⌋ :=
+  by
+    intro n Γ' A b B hbB ihbB m l Γ Δ heqM S t T hS heqΓ heqt heqT
+    cases heqM
+    cases heqΓ
+    cases heqt
+    cases heqT
+    apply HasType.pi_intro
+    rw [extend_expand_context_weaken_from]
+    simp [lift_weak_n]
+    rw [lift_weaken_from]
+    apply ihbB
+    apply hS
+    repeat' rfl
+    apply gen_ctx_leq Δ
+
+theorem weakening_sigma_intro :
+    ∀ {n : Nat} {Γ : Ctx n} {a A b : Tm n} {B : Tm (n + 1)},
+      (Γ ⊢ a ∶ A) →
+        (Γ ⊢ b ∶ B⌈a⌉₀) →
+          Γ ⬝ A ⊢ B type →
+            (∀ (m l : Nat) (Γ_1 : Ctx l) (Δ : CtxGen l m) (eqM : n = m) (S : Tm l) (a_4 A_1 : Tm m),
+                Γ_1 ⊢ S type →
+                  eqM ▸ Γ = Γ_1 ⊗ Δ → eqM ▸ a = a_4 → eqM ▸ A = A_1 → (Γ_1 ⬝ S ⊗ ⌊↑₁↬l⌋Δ) ⊢ a_4⌊↑₁m↬l⌋ ∶ A_1⌊↑₁m↬l⌋) →
+              (∀ (m l : Nat) (Γ_1 : Ctx l) (Δ : CtxGen l m) (eqM : n = m) (S : Tm l) (a_5 A : Tm m),
+                  Γ_1 ⊢ S type →
+                    eqM ▸ Γ = Γ_1 ⊗ Δ → eqM ▸ b = a_5 → eqM ▸ B⌈a⌉₀ = A → (Γ_1 ⬝ S ⊗ ⌊↑₁↬l⌋Δ) ⊢ a_5⌊↑₁m↬l⌋ ∶ A⌊↑₁m↬l⌋) →
+                (∀ (m l : Nat) (Γ_1 : Ctx l) (Δ : CtxGen l m) (eqM : n + 1 = m) (S : Tm l) (A_1 : Tm m),
+                    Γ_1 ⊢ S type → eqM ▸ Γ ⬝ A = Γ_1 ⊗ Δ → eqM ▸ B = A_1 → (Γ_1 ⬝ S ⊗ ⌊↑₁↬l⌋Δ) ⊢ A_1⌊↑₁m↬l⌋ type) →
+                  ∀ (m l : Nat) (Γ_1 : Ctx l) (Δ : CtxGen l m) (eqM : n = m) (S : Tm l) (a_7 A_1 : Tm m),
+                    Γ_1 ⊢ S type →
+                      eqM ▸ Γ = Γ_1 ⊗ Δ →
+                        eqM ▸ a&b = a_7 → (eqM ▸ ΣA;B) = A_1 → (Γ_1 ⬝ S ⊗ ⌊↑₁↬l⌋Δ) ⊢ a_7⌊↑₁m↬l⌋ ∶ A_1⌊↑₁m↬l⌋ :=
+  by
+    intro n Γ a A b B haA hbB hB ihaA ihbB ihB m l Γ Δ heqM S t T hS heqΓ heqt heqT
+    cases heqM
+    cases heqΓ
+    cases heqt
+    cases heqT
+    apply HasType.sigma_intro
+    · apply ihaA
+      apply hS
+      repeat' rfl
+    · simp [lift_weak_n]
+      simp [←weak_sub_zero]
+      apply ihbB
+      apply hS
+      repeat' rfl
+    · simp [lift_weak_n]
+      rw [lift_weaken_from]
+      rw [extend_expand_context_weaken_from]
+      apply ihB
+      apply hS
+      repeat' rfl
+      apply gen_ctx_leq Δ
+
+theorem weakening_nat_zero_intro :
+    ∀ {n : Nat} {Γ : Ctx n},
+      Γ ctx →
+        (∀ (m l : Nat) (Γ_1 : Ctx l) (Δ : CtxGen l m) (eqM : n = m) (S : Tm l),
+            Γ_1 ⊢ S type → eqM ▸ Γ = Γ_1 ⊗ Δ → (Γ_1 ⬝ S ⊗ ⌊↑₁↬l⌋Δ) ctx) →
+          ∀ (m l : Nat) (Γ_1 : Ctx l) (Δ : CtxGen l m) (eqM : n = m) (S : Tm l) (a A : Tm m),
+            Γ_1 ⊢ S type → eqM ▸ Γ = Γ_1 ⊗ Δ → eqM ▸ 𝓏 = a → eqM ▸ 𝒩 = A → (Γ_1 ⬝ S ⊗ ⌊↑₁↬l⌋Δ) ⊢ a⌊↑₁m↬l⌋ ∶ A⌊↑₁m↬l⌋ :=
+  by
+    intro n Γ hiC ihiC m l Γ Δ heqM S t T hS heqΓ heqt heqT
+    cases heqM
+    cases heqΓ
+    cases heqt
+    cases heqT
+    apply HasType.nat_zero_intro
+    apply ihiC
+    apply hS
+    repeat' rfl
+
+theorem weakening_nat_succ_intro :
+    ∀ {n : Nat} {Γ : Ctx n} {x : Tm n},
+      (Γ ⊢ x ∶ 𝒩) →
+        (∀ (m l : Nat) (Γ_1 : Ctx l) (Δ : CtxGen l m) (eqM : n = m) (S : Tm l) (a A : Tm m),
+            Γ_1 ⊢ S type → eqM ▸ Γ = Γ_1 ⊗ Δ → eqM ▸ x = a → eqM ▸ 𝒩 = A → (Γ_1 ⬝ S ⊗ ⌊↑₁↬l⌋Δ) ⊢ a⌊↑₁m↬l⌋ ∶ A⌊↑₁m↬l⌋) →
+          ∀ (m l : Nat) (Γ_1 : Ctx l) (Δ : CtxGen l m) (eqM : n = m) (S : Tm l) (a A : Tm m),
+            Γ_1 ⊢ S type → eqM ▸ Γ = Γ_1 ⊗ Δ → eqM ▸ 𝓈(x) = a → eqM ▸ 𝒩 = A → (Γ_1 ⬝ S ⊗ ⌊↑₁↬l⌋Δ) ⊢ a⌊↑₁m↬l⌋ ∶ A⌊↑₁m↬l⌋ :=
+  by
+    intro n Γ x hxNat ihxNat m l Γ Δ heqM S t T hS heqΓ heqt heqT
+    cases heqM
+    cases heqΓ
+    cases heqt
+    cases heqT
+    apply HasType.nat_succ_intro
+    rw [←weakening_nat]
+    apply ihxNat
+    apply hS
+    repeat' rfl
+
+theorem weakening_iden_intro :
+    ∀ {n : Nat} {Γ : Ctx n} {A a : Tm n},
+      Γ ⊢ A type →
+        (Γ ⊢ a ∶ A) →
+          (∀ (m l : Nat) (Γ_1 : Ctx l) (Δ : CtxGen l m) (eqM : n = m) (S : Tm l) (A_1 : Tm m),
+              Γ_1 ⊢ S type → eqM ▸ Γ = Γ_1 ⊗ Δ → eqM ▸ A = A_1 → (Γ_1 ⬝ S ⊗ ⌊↑₁↬l⌋Δ) ⊢ A_1⌊↑₁m↬l⌋ type) →
+            (∀ (m l : Nat) (Γ_1 : Ctx l) (Δ : CtxGen l m) (eqM : n = m) (S : Tm l) (a_4 A_1 : Tm m),
+                Γ_1 ⊢ S type →
+                  eqM ▸ Γ = Γ_1 ⊗ Δ → eqM ▸ a = a_4 → eqM ▸ A = A_1 → (Γ_1 ⬝ S ⊗ ⌊↑₁↬l⌋Δ) ⊢ a_4⌊↑₁m↬l⌋ ∶ A_1⌊↑₁m↬l⌋) →
+              ∀ (m l : Nat) (Γ_1 : Ctx l) (Δ : CtxGen l m) (eqM : n = m) (S : Tm l) (a_5 A_1 : Tm m),
+                Γ_1 ⊢ S type →
+                  eqM ▸ Γ = Γ_1 ⊗ Δ →
+                    eqM ▸ A.refl a = a_5 → (eqM ▸ a ≃[A] a) = A_1 → (Γ_1 ⬝ S ⊗ ⌊↑₁↬l⌋Δ) ⊢ a_5⌊↑₁m↬l⌋ ∶ A_1⌊↑₁m↬l⌋ :=
+  by
+    intro n Γ A a hA haA ihA ihaA m l Γ Δ heqM S t T hS heqΓ heqt heqT
+    cases heqM
+    cases heqΓ
+    cases heqt
+    cases heqT
+    apply HasType.iden_intro
+    · apply ihA
+      apply hS
+      repeat' rfl
+    · apply ihaA
+      apply hS
+      repeat' rfl
+
+theorem weakening_univ_unit :
+    ∀ {n : Nat} {Γ : Ctx n},
+      Γ ctx →
+        (∀ (m l : Nat) (Γ_1 : Ctx l) (Δ : CtxGen l m) (eqM : n = m) (S : Tm l),
+            Γ_1 ⊢ S type → eqM ▸ Γ = Γ_1 ⊗ Δ → (Γ_1 ⬝ S ⊗ ⌊↑₁↬l⌋Δ) ctx) →
+          ∀ (m l : Nat) (Γ_1 : Ctx l) (Δ : CtxGen l m) (eqM : n = m) (S : Tm l) (a A : Tm m),
+            Γ_1 ⊢ S type → eqM ▸ Γ = Γ_1 ⊗ Δ → eqM ▸ 𝟙 = a → eqM ▸ 𝒰 = A → (Γ_1 ⬝ S ⊗ ⌊↑₁↬l⌋Δ) ⊢ a⌊↑₁m↬l⌋ ∶ A⌊↑₁m↬l⌋ :=
+  by
+    intro n Γ hiC ihiC m l Γ Δ heqM S t T hS heqΓ heqt heqT
+    cases heqM
+    cases heqΓ
+    cases heqt
+    cases heqT
+    apply HasType.univ_unit
+    apply ihiC
+    apply hS
+    repeat' rfl
+
+theorem weakening_univ_empty :
+    ∀ {n : Nat} {Γ : Ctx n},
+      Γ ctx →
+        (∀ (m l : Nat) (Γ_1 : Ctx l) (Δ : CtxGen l m) (eqM : n = m) (S : Tm l),
+            Γ_1 ⊢ S type → eqM ▸ Γ = Γ_1 ⊗ Δ → (Γ_1 ⬝ S ⊗ ⌊↑₁↬l⌋Δ) ctx) →
+          ∀ (m l : Nat) (Γ_1 : Ctx l) (Δ : CtxGen l m) (eqM : n = m) (S : Tm l) (a A : Tm m),
+            Γ_1 ⊢ S type → eqM ▸ Γ = Γ_1 ⊗ Δ → eqM ▸ 𝟘 = a → eqM ▸ 𝒰 = A → (Γ_1 ⬝ S ⊗ ⌊↑₁↬l⌋Δ) ⊢ a⌊↑₁m↬l⌋ ∶ A⌊↑₁m↬l⌋ :=
+  by
+    intro n Γ hiC ihiC m l Γ Δ heqM S t T hS heqΓ heqt heqT
+    cases heqM
+    cases heqΓ
+    cases heqt
+    cases heqT
+    apply HasType.univ_empty
+    apply ihiC
+    apply hS
+    repeat' rfl
+
+theorem weakening_univ_pi :
+    ∀ {n : Nat} {Γ : Ctx n} {A : Tm n} {B : Tm (n + 1)},
+      (Γ ⊢ A ∶ 𝒰) →
+        (Γ ⬝ A ⊢ B ∶ 𝒰) →
+          (∀ (m l : Nat) (Γ_1 : Ctx l) (Δ : CtxGen l m) (eqM : n = m) (S : Tm l) (a A_1 : Tm m),
+              Γ_1 ⊢ S type →
+                eqM ▸ Γ = Γ_1 ⊗ Δ → eqM ▸ A = a → eqM ▸ 𝒰 = A_1 → (Γ_1 ⬝ S ⊗ ⌊↑₁↬l⌋Δ) ⊢ a⌊↑₁m↬l⌋ ∶ A_1⌊↑₁m↬l⌋) →
+            (∀ (m l : Nat) (Γ_1 : Ctx l) (Δ : CtxGen l m) (eqM : n + 1 = m) (S : Tm l) (a A_1 : Tm m),
+                Γ_1 ⊢ S type →
+                  eqM ▸ Γ ⬝ A = Γ_1 ⊗ Δ → eqM ▸ B = a → eqM ▸ 𝒰 = A_1 → (Γ_1 ⬝ S ⊗ ⌊↑₁↬l⌋Δ) ⊢ a⌊↑₁m↬l⌋ ∶ A_1⌊↑₁m↬l⌋) →
+              ∀ (m l : Nat) (Γ_1 : Ctx l) (Δ : CtxGen l m) (eqM : n = m) (S : Tm l) (a A_1 : Tm m),
+                Γ_1 ⊢ S type →
+                  eqM ▸ Γ = Γ_1 ⊗ Δ → (eqM ▸ ΠA;B) = a → eqM ▸ 𝒰 = A_1 → (Γ_1 ⬝ S ⊗ ⌊↑₁↬l⌋Δ) ⊢ a⌊↑₁m↬l⌋ ∶ A_1⌊↑₁m↬l⌋ :=
+  by
+    intro n Γ A B hAU hBU ihAU ihBU m l Γ Δ heqM S t T hS heqΓ heqt heqT
+    cases heqM
+    cases heqΓ
+    cases heqt
+    cases heqT
+    apply HasType.univ_pi
+    · rw [←weakening_univ]
+      apply ihAU
+      apply hS
+      repeat' rfl
+    · rw [←weakening_univ]
+      rw [extend_expand_context_weaken_from]
+      simp [lift_weak_n]
+      rw [lift_weaken_from]
+      apply ihBU
+      apply hS
+      repeat' rfl
+      apply gen_ctx_leq Δ
+
+theorem weakening_univ_sigma :
+    ∀ {n : Nat} {Γ : Ctx n} {A : Tm n} {B : Tm (n + 1)},
+      (Γ ⊢ A ∶ 𝒰) →
+        (Γ ⬝ A ⊢ B ∶ 𝒰) →
+          (∀ (m l : Nat) (Γ_1 : Ctx l) (Δ : CtxGen l m) (eqM : n = m) (S : Tm l) (a A_1 : Tm m),
+              Γ_1 ⊢ S type →
+                eqM ▸ Γ = Γ_1 ⊗ Δ → eqM ▸ A = a → eqM ▸ 𝒰 = A_1 → (Γ_1 ⬝ S ⊗ ⌊↑₁↬l⌋Δ) ⊢ a⌊↑₁m↬l⌋ ∶ A_1⌊↑₁m↬l⌋) →
+            (∀ (m l : Nat) (Γ_1 : Ctx l) (Δ : CtxGen l m) (eqM : n + 1 = m) (S : Tm l) (a A_1 : Tm m),
+                Γ_1 ⊢ S type →
+                  eqM ▸ Γ ⬝ A = Γ_1 ⊗ Δ → eqM ▸ B = a → eqM ▸ 𝒰 = A_1 → (Γ_1 ⬝ S ⊗ ⌊↑₁↬l⌋Δ) ⊢ a⌊↑₁m↬l⌋ ∶ A_1⌊↑₁m↬l⌋) →
+              ∀ (m l : Nat) (Γ_1 : Ctx l) (Δ : CtxGen l m) (eqM : n = m) (S : Tm l) (a A_1 : Tm m),
+                Γ_1 ⊢ S type →
+                  eqM ▸ Γ = Γ_1 ⊗ Δ → (eqM ▸ ΣA;B) = a → eqM ▸ 𝒰 = A_1 → (Γ_1 ⬝ S ⊗ ⌊↑₁↬l⌋Δ) ⊢ a⌊↑₁m↬l⌋ ∶ A_1⌊↑₁m↬l⌋ :=
+  by
+    intro n Γ A B hAU hBU ihAU ihBU m l Γ Δ heqM S t T hS heqΓ heqt heqT
+    cases heqM
+    cases heqΓ
+    cases heqt
+    cases heqT
+    apply HasType.univ_sigma
+    · rw [←weakening_univ]
+      apply ihAU
+      apply hS
+      repeat' rfl
+    · rw [←weakening_univ]
+      rw [extend_expand_context_weaken_from]
+      simp [lift_weak_n]
+      rw [lift_weaken_from]
+      apply ihBU
+      apply hS
+      repeat' rfl
+      apply gen_ctx_leq Δ
+
+theorem weakening_univ_nat :
+    ∀ {n : Nat} {Γ : Ctx n},
+      Γ ctx →
+        (∀ (m l : Nat) (Γ_1 : Ctx l) (Δ : CtxGen l m) (eqM : n = m) (S : Tm l),
+            Γ_1 ⊢ S type → eqM ▸ Γ = Γ_1 ⊗ Δ → (Γ_1 ⬝ S ⊗ ⌊↑₁↬l⌋Δ) ctx) →
+          ∀ (m l : Nat) (Γ_1 : Ctx l) (Δ : CtxGen l m) (eqM : n = m) (S : Tm l) (a A : Tm m),
+            Γ_1 ⊢ S type → eqM ▸ Γ = Γ_1 ⊗ Δ → eqM ▸ 𝒩 = a → eqM ▸ 𝒰 = A → (Γ_1 ⬝ S ⊗ ⌊↑₁↬l⌋Δ) ⊢ a⌊↑₁m↬l⌋ ∶ A⌊↑₁m↬l⌋ :=
+  by
+    intro n Γ hiC ihiC m l Γ Δ heqM S t T hS heqΓ heqt heqT
+    cases heqM
+    cases heqΓ
+    cases heqt
+    cases heqT
+    apply HasType.univ_nat
+    apply ihiC
+    apply hS
+    repeat' rfl
+
+theorem weakening_univ_iden :
+    ∀ {n : Nat} {Γ : Ctx n} {A a a' : Tm n},
+      (Γ ⊢ A ∶ 𝒰) →
+        (Γ ⊢ a ∶ A) →
+          (Γ ⊢ a' ∶ A) →
+            (∀ (m l : Nat) (Γ_1 : Ctx l) (Δ : CtxGen l m) (eqM : n = m) (S : Tm l) (a A_1 : Tm m),
+                Γ_1 ⊢ S type →
+                  eqM ▸ Γ = Γ_1 ⊗ Δ → eqM ▸ A = a → eqM ▸ 𝒰 = A_1 → (Γ_1 ⬝ S ⊗ ⌊↑₁↬l⌋Δ) ⊢ a⌊↑₁m↬l⌋ ∶ A_1⌊↑₁m↬l⌋) →
+              (∀ (m l : Nat) (Γ_1 : Ctx l) (Δ : CtxGen l m) (eqM : n = m) (S : Tm l) (a_5 A_1 : Tm m),
+                  Γ_1 ⊢ S type →
+                    eqM ▸ Γ = Γ_1 ⊗ Δ → eqM ▸ a = a_5 → eqM ▸ A = A_1 → (Γ_1 ⬝ S ⊗ ⌊↑₁↬l⌋Δ) ⊢ a_5⌊↑₁m↬l⌋ ∶ A_1⌊↑₁m↬l⌋) →
+                (∀ (m l : Nat) (Γ_1 : Ctx l) (Δ : CtxGen l m) (eqM : n = m) (S : Tm l) (a A_1 : Tm m),
+                    Γ_1 ⊢ S type →
+                      eqM ▸ Γ = Γ_1 ⊗ Δ → eqM ▸ a' = a → eqM ▸ A = A_1 → (Γ_1 ⬝ S ⊗ ⌊↑₁↬l⌋Δ) ⊢ a⌊↑₁m↬l⌋ ∶ A_1⌊↑₁m↬l⌋) →
+                  ∀ (m l : Nat) (Γ_1 : Ctx l) (Δ : CtxGen l m) (eqM : n = m) (S : Tm l) (a_7 A_1 : Tm m),
+                    Γ_1 ⊢ S type →
+                      eqM ▸ Γ = Γ_1 ⊗ Δ →
+                        (eqM ▸ a ≃[A] a') = a_7 → eqM ▸ 𝒰 = A_1 → (Γ_1 ⬝ S ⊗ ⌊↑₁↬l⌋Δ) ⊢ a_7⌊↑₁m↬l⌋ ∶ A_1⌊↑₁m↬l⌋ :=
+  by
+    intro n Γ A a a' hAU haA haA' ihAU ihaA ihaA' m l Γ Δ heqM S t T hS heqΓ heqt heqT
+    cases heqM
+    cases heqΓ
+    cases heqt
+    cases heqT
+    apply HasType.univ_iden
+    · rw [←weakening_univ]
+      apply ihAU
+      apply hS
+      repeat' rfl
+    · apply ihaA
+      apply hS
+      repeat' rfl
+    · apply ihaA'
+      apply hS
+      repeat' rfl
+
+theorem weakening_unit_elim :
+    ∀ {n : Nat} {Γ : Ctx n} {A : Tm (n + 1)} {a b : Tm n},
+      Γ ⬝ 𝟙 ⊢ A type →
+        (Γ ⊢ a ∶ A⌈⋆⌉₀) →
+          (Γ ⊢ b ∶ 𝟙) →
+            (∀ (m l : Nat) (Γ_1 : Ctx l) (Δ : CtxGen l m) (eqM : n + 1 = m) (S : Tm l) (A_1 : Tm m),
+                Γ_1 ⊢ S type → eqM ▸ Γ ⬝ 𝟙 = Γ_1 ⊗ Δ → eqM ▸ A = A_1 → (Γ_1 ⬝ S ⊗ ⌊↑₁↬l⌋Δ) ⊢ A_1⌊↑₁m↬l⌋ type) →
+              (∀ (m l : Nat) (Γ_1 : Ctx l) (Δ : CtxGen l m) (eqM : n = m) (S : Tm l) (a_5 A_1 : Tm m),
+                  Γ_1 ⊢ S type →
+                    eqM ▸ Γ = Γ_1 ⊗ Δ → eqM ▸ a = a_5 → eqM ▸ A⌈⋆⌉₀ = A_1 → (Γ_1 ⬝ S ⊗ ⌊↑₁↬l⌋Δ) ⊢ a_5⌊↑₁m↬l⌋ ∶ A_1⌊↑₁m↬l⌋) →
+                (∀ (m l : Nat) (Γ_1 : Ctx l) (Δ : CtxGen l m) (eqM : n = m) (S : Tm l) (a A : Tm m),
+                    Γ_1 ⊢ S type →
+                      eqM ▸ Γ = Γ_1 ⊗ Δ → eqM ▸ b = a → eqM ▸ 𝟙 = A → (Γ_1 ⬝ S ⊗ ⌊↑₁↬l⌋Δ) ⊢ a⌊↑₁m↬l⌋ ∶ A⌊↑₁m↬l⌋) →
+                  ∀ (m l : Nat) (Γ_1 : Ctx l) (Δ : CtxGen l m) (eqM : n = m) (S : Tm l) (a_7 A_1 : Tm m),
+                    Γ_1 ⊢ S type →
+                      eqM ▸ Γ = Γ_1 ⊗ Δ →
+                        eqM ▸ A.indUnit b a = a_7 → eqM ▸ A⌈b⌉₀ = A_1 → (Γ_1 ⬝ S ⊗ ⌊↑₁↬l⌋Δ) ⊢ a_7⌊↑₁m↬l⌋ ∶ A_1⌊↑₁m↬l⌋ :=
+  by
+    intro n Γ A a b hA haA hb1 ihA ihaA ihb1 m l Γ Δ heqM S t T hS heqΓ heqt heqT
+    cases heqM
+    cases heqΓ
+    cases heqt
+    cases heqT
+    rw [weak_sub_zero]
+    apply HasType.unit_elim
+    · rw [←weakening_unit]
+      rw [extend_expand_context_weaken_from]
+      simp [lift_weak_n]
+      rw [lift_weaken_from]
+      apply ihA
+      apply hS
+      repeat' rfl
+      apply gen_ctx_leq Δ
+    · rw [←weakening_tt]
+      simp [lift_weak_n]
+      rw [←weak_sub_zero]
+      apply ihaA
+      apply hS
+      repeat' rfl
+    · rw [←weakening_unit]
+      apply ihb1
+      apply hS
+      repeat' rfl
+
+theorem weakening_empty_elim :
+    ∀ {n : Nat} {Γ : Ctx n} {A : Tm (n + 1)} {b : Tm n},
+      Γ ⬝ 𝟘 ⊢ A type →
+        (Γ ⊢ b ∶ 𝟘) →
+          (∀ (m l : Nat) (Γ_1 : Ctx l) (Δ : CtxGen l m) (eqM : n + 1 = m) (S : Tm l) (A_1 : Tm m),
+              Γ_1 ⊢ S type → eqM ▸ Γ ⬝ 𝟘 = Γ_1 ⊗ Δ → eqM ▸ A = A_1 → (Γ_1 ⬝ S ⊗ ⌊↑₁↬l⌋Δ) ⊢ A_1⌊↑₁m↬l⌋ type) →
+            (∀ (m l : Nat) (Γ_1 : Ctx l) (Δ : CtxGen l m) (eqM : n = m) (S : Tm l) (a A : Tm m),
+                Γ_1 ⊢ S type → eqM ▸ Γ = Γ_1 ⊗ Δ → eqM ▸ b = a → eqM ▸ 𝟘 = A → (Γ_1 ⬝ S ⊗ ⌊↑₁↬l⌋Δ) ⊢ a⌊↑₁m↬l⌋ ∶ A⌊↑₁m↬l⌋) →
+              ∀ (m l : Nat) (Γ_1 : Ctx l) (Δ : CtxGen l m) (eqM : n = m) (S : Tm l) (a A_1 : Tm m),
+                Γ_1 ⊢ S type →
+                  eqM ▸ Γ = Γ_1 ⊗ Δ →
+                    eqM ▸ A.indEmpty b = a → eqM ▸ A⌈b⌉₀ = A_1 → (Γ_1 ⬝ S ⊗ ⌊↑₁↬l⌋Δ) ⊢ a⌊↑₁m↬l⌋ ∶ A_1⌊↑₁m↬l⌋ :=
+  by
+    intro n Γ A b hA hb0 ihA ihb0 m l Γ Δ heqM S t T hS heqΓ heqt heqT
+    cases heqM
+    cases heqΓ
+    cases heqt
+    cases heqT
+    rw [weak_sub_zero]
+    apply HasType.empty_elim
+    · rw [←weakening_empty]
+      rw [extend_expand_context_weaken_from]
+      simp [lift_weak_n]
+      rw [lift_weaken_from]
+      apply ihA
+      apply hS
+      repeat' rfl
+      apply gen_ctx_leq Δ
+    · rw [←weakening_empty]
+      apply ihb0
+      apply hS
+      repeat' rfl
+
+theorem weakening_pi_elim :
+    ∀ {n : Nat} {Γ : Ctx n} {f A : Tm n} {B : Tm (n + 1)} {a : Tm n},
+      (Γ ⊢ f ∶ ΠA;B) →
+        (Γ ⊢ a ∶ A) →
+          (∀ (m l : Nat) (Γ_1 : Ctx l) (Δ : CtxGen l m) (eqM : n = m) (S : Tm l) (a A_1 : Tm m),
+              Γ_1 ⊢ S type →
+                eqM ▸ Γ = Γ_1 ⊗ Δ → eqM ▸ f = a → (eqM ▸ ΠA;B) = A_1 → (Γ_1 ⬝ S ⊗ ⌊↑₁↬l⌋Δ) ⊢ a⌊↑₁m↬l⌋ ∶ A_1⌊↑₁m↬l⌋) →
+            (∀ (m l : Nat) (Γ_1 : Ctx l) (Δ : CtxGen l m) (eqM : n = m) (S : Tm l) (a_4 A_1 : Tm m),
+                Γ_1 ⊢ S type →
+                  eqM ▸ Γ = Γ_1 ⊗ Δ → eqM ▸ a = a_4 → eqM ▸ A = A_1 → (Γ_1 ⬝ S ⊗ ⌊↑₁↬l⌋Δ) ⊢ a_4⌊↑₁m↬l⌋ ∶ A_1⌊↑₁m↬l⌋) →
+              ∀ (m l : Nat) (Γ_1 : Ctx l) (Δ : CtxGen l m) (eqM : n = m) (S : Tm l) (a_5 A : Tm m),
+                Γ_1 ⊢ S type →
+                  eqM ▸ Γ = Γ_1 ⊗ Δ → eqM ▸ f◃a = a_5 → eqM ▸ B⌈a⌉₀ = A → (Γ_1 ⬝ S ⊗ ⌊↑₁↬l⌋Δ) ⊢ a_5⌊↑₁m↬l⌋ ∶ A⌊↑₁m↬l⌋ :=
+  by
+    intro n Γ f A B a hfPi haA ihfPi ihaA m l Γ Δ heqM S t T hS heqΓ heqt heqT
+    cases heqM
+    cases heqΓ
+    cases heqt
+    cases heqT
+    rw [weak_sub_zero]
+    apply HasType.pi_elim
+    · rw [←weakening_pi]
+      apply ihfPi
+      apply hS
+      repeat' rfl
+    · apply ihaA
+      apply hS
+      repeat' rfl
+
+theorem weakening_sigma_elim :
+    ∀ {n : Nat} {Γ : Ctx n} {A : Tm n} {B : Tm (n + 1)} {p : Tm n} {C : Tm (n + 1)} {c : Tm (n + 1 + 1)},
+    (Γ ⊢ p ∶ ΣA;B) →
+      (Γ ⬝ ΣA;B) ⊢ C type →
+        (Γ ⬝ A ⬝ B ⊢ c ∶ C⌈(ₛ↑ₚ↑ₚidₚ), v(1)&v(0)⌉) →
+          (∀ (m l : Nat) (Γ_1 : Ctx l) (Δ : CtxGen l m) (eqM : n = m) (S : Tm l) (a A_1 : Tm m),
+              Γ_1 ⊢ S type →
+                eqM ▸ Γ = Γ_1 ⊗ Δ → eqM ▸ p = a → (eqM ▸ ΣA;B) = A_1 → (Γ_1 ⬝ S ⊗ ⌊↑₁↬l⌋Δ) ⊢ a⌊↑₁m↬l⌋ ∶ A_1⌊↑₁m↬l⌋) →
+            (∀ (m l : Nat) (Γ_1 : Ctx l) (Δ : CtxGen l m) (eqM : n + 1 = m) (S : Tm l) (A_1 : Tm m),
+                Γ_1 ⊢ S type → (eqM ▸ Γ ⬝ ΣA;B) = Γ_1 ⊗ Δ → eqM ▸ C = A_1 → (Γ_1 ⬝ S ⊗ ⌊↑₁↬l⌋Δ) ⊢ A_1⌊↑₁m↬l⌋ type) →
+              (∀ (m l : Nat) (Γ_1 : Ctx l) (Δ : CtxGen l m) (eqM : n + 1 + 1 = m) (S : Tm l) (a A_1 : Tm m),
+                  Γ_1 ⊢ S type →
+                    eqM ▸ Γ ⬝ A ⬝ B = Γ_1 ⊗ Δ →
+                      eqM ▸ c = a → eqM ▸ C⌈(ₛ↑ₚ↑ₚidₚ), v(1)&v(0)⌉ = A_1 → (Γ_1 ⬝ S ⊗ ⌊↑₁↬l⌋Δ) ⊢ a⌊↑₁m↬l⌋ ∶ A_1⌊↑₁m↬l⌋) →
+                ∀ (m l : Nat) (Γ_1 : Ctx l) (Δ : CtxGen l m) (eqM : n = m) (S : Tm l) (a A_1 : Tm m),
+                  Γ_1 ⊢ S type →
+                    eqM ▸ Γ = Γ_1 ⊗ Δ →
+                      eqM ▸ A.indSigma B C c p = a → eqM ▸ C⌈p⌉₀ = A_1 → (Γ_1 ⬝ S ⊗ ⌊↑₁↬l⌋Δ) ⊢ a⌊↑₁m↬l⌋ ∶ A_1⌊↑₁m↬l⌋ :=
+  by
+    intro n Γ A B p C c hpSi hC hcC ihpSi ihC ihcC m l Γ Δ heqM S t T hS heqΓ heqt heqT
+    cases heqM
+    cases heqΓ
+    cases heqt
+    cases heqT
+    rw [weak_sub_zero]
+    apply HasType.sigma_elim
+    · simp [lift_weak_n]
+      rw [←weakening_sigma]
+      apply ihpSi
+      apply hS
+      repeat' rfl
+    · simp [lift_weak_n]
+      rw [←weakening_sigma]
+      rw [lift_weaken_from]
+      rw [extend_expand_context_weaken_from]
+      apply ihC
+      apply hS
+      repeat' rfl
+      apply  gen_ctx_leq Δ
+    · have h := gen_ctx_leq Δ
+      simp [lift_weak_n]
+      rw [lift_weaken_from]
+      rw [lift_weaken_from]
+      simp [extend_expand_context_weaken_from]
+      rw [weak_subst_sigma_C]
+      apply ihcC
+      apply hS
+      repeat' rfl
+      any_goals omega
+
+theorem weakening_nat_elim :
+    ∀ {n : Nat} {Γ : Ctx n} {z x : Tm n} {A : Tm (n + 1)} {s : Tm (n + 2)},
+      Γ ⬝ 𝒩 ⊢ A type →
+        (Γ ⊢ z ∶ A⌈𝓏⌉₀) →
+          (Γ ⬝ 𝒩 ⬝ A ⊢ s ∶ A⌈(ₛ↑ₚidₚ), 𝓈(v(0))⌉⌊↑ₚidₚ⌋) →
+            (Γ ⊢ x ∶ 𝒩) →
+              (∀ (m l : Nat) (Γ_1 : Ctx l) (Δ : CtxGen l m) (eqM : n + 1 = m) (S : Tm l) (A_1 : Tm m),
+                  Γ_1 ⊢ S type → eqM ▸ Γ ⬝ 𝒩 = Γ_1 ⊗ Δ → eqM ▸ A = A_1 → (Γ_1 ⬝ S ⊗ ⌊↑₁↬l⌋Δ) ⊢ A_1⌊↑₁m↬l⌋ type) →
+                (∀ (m l : Nat) (Γ_1 : Ctx l) (Δ : CtxGen l m) (eqM : n = m) (S : Tm l) (a A_1 : Tm m),
+                    Γ_1 ⊢ S type →
+                      eqM ▸ Γ = Γ_1 ⊗ Δ → eqM ▸ z = a → eqM ▸ A⌈𝓏⌉₀ = A_1 → (Γ_1 ⬝ S ⊗ ⌊↑₁↬l⌋Δ) ⊢ a⌊↑₁m↬l⌋ ∶ A_1⌊↑₁m↬l⌋) →
+                  (∀ (m l : Nat) (Γ_1 : Ctx l) (Δ : CtxGen l m) (eqM : n + 1 + 1 = m) (S : Tm l) (a A_1 : Tm m),
+                      Γ_1 ⊢ S type →
+                        eqM ▸ Γ ⬝ 𝒩 ⬝ A = Γ_1 ⊗ Δ →
+                          eqM ▸ s = a →
+                            eqM ▸ A⌈(ₛ↑ₚidₚ), 𝓈(v(0))⌉⌊↑ₚidₚ⌋ = A_1 → (Γ_1 ⬝ S ⊗ ⌊↑₁↬l⌋Δ) ⊢ a⌊↑₁m↬l⌋ ∶ A_1⌊↑₁m↬l⌋) →
+                    (∀ (m l : Nat) (Γ_1 : Ctx l) (Δ : CtxGen l m) (eqM : n = m) (S : Tm l) (a A : Tm m),
+                        Γ_1 ⊢ S type →
+                          eqM ▸ Γ = Γ_1 ⊗ Δ → eqM ▸ x = a → eqM ▸ 𝒩 = A → (Γ_1 ⬝ S ⊗ ⌊↑₁↬l⌋Δ) ⊢ a⌊↑₁m↬l⌋ ∶ A⌊↑₁m↬l⌋) →
+                      ∀ (m l : Nat) (Γ_1 : Ctx l) (Δ : CtxGen l m) (eqM : n = m) (S : Tm l) (a A_1 : Tm m),
+                        Γ_1 ⊢ S type →
+                          eqM ▸ Γ = Γ_1 ⊗ Δ →
+                            eqM ▸ A.indNat z s x = a → eqM ▸ A⌈x⌉₀ = A_1 → (Γ_1 ⬝ S ⊗ ⌊↑₁↬l⌋Δ) ⊢ a⌊↑₁m↬l⌋ ∶ A_1⌊↑₁m↬l⌋ :=
+  by
+    intro n Γ z x A s hA hzA hsA hxA ihA ihzA ihsA ihxA m l Γ Δ heqM S t T hS heqΓ heqt heqT
+    cases heqM
+    cases heqΓ
+    cases heqt
+    cases heqT
+    rw [weak_sub_zero]
+    apply HasType.nat_elim
+    · rw [←weakening_nat]
+      rw [extend_expand_context_weaken_from]
+      simp [lift_weak_n]
+      rw [lift_weaken_from]
+      apply ihA
+      apply hS
+      repeat' rfl
+      apply gen_ctx_leq Δ
+    · rw [←weakening_nat_zero]
+      simp [lift_weak_n]
+      rw [←weak_sub_zero]
+      apply ihzA
+      apply hS
+      repeat' rfl
+    · have h := gen_ctx_leq Δ
+      rw [←weakening_nat]
+      rw [←helper_weak_nat_succ]
+      rw [extend_expand_context_weaken_from]
+      simp [lift_weak_n]
+      rw [lift_weaken_from]
+      rw [lift_weaken_from]
+      rw [extend_expand_context_weaken_from]
+      apply ihsA
+      apply hS
+      repeat' rfl
+      any_goals omega
+    · rw [←weakening_nat]
+      apply ihxA
+      apply hS
+      repeat' rfl
+
+theorem weakening_iden_elim :
+    ∀ {n : Nat} {Γ : Ctx n} {A : Tm n} {B : Tm (n + 1 + 1 + 1)} {b : Tm (n + 1)} {a a' p : Tm n},
+    (Γ ⬝ A ⬝ A⌊↑ₚidₚ⌋ ⬝ v(1) ≃[A⌊↑ₚ↑ₚidₚ⌋] v(0)) ⊢ B type →
+      (Γ ⬝ A ⊢ b ∶ B⌈(ₛidₚ), v(0), (A⌊↑ₚidₚ⌋.refl v(0))⌉) →
+        (Γ ⊢ a ∶ A) →
+          (Γ ⊢ a' ∶ A) →
+            (Γ ⊢ p ∶ a ≃[A] a') →
+              (∀ (m l : Nat) (Γ_1 : Ctx l) (Δ : CtxGen l m) (eqM : n + 1 + 1 + 1 = m) (S : Tm l) (A_1 : Tm m),
+                  Γ_1 ⊢ S type →
+                    (eqM ▸ Γ ⬝ A ⬝ A⌊↑ₚidₚ⌋ ⬝ v(1) ≃[A⌊↑ₚ↑ₚidₚ⌋] v(0)) = Γ_1 ⊗ Δ →
+                      eqM ▸ B = A_1 → (Γ_1 ⬝ S ⊗ ⌊↑₁↬l⌋Δ) ⊢ A_1⌊↑₁m↬l⌋ type) →
+                (∀ (m l : Nat) (Γ_1 : Ctx l) (Δ : CtxGen l m) (eqM : n + 1 = m) (S : Tm l) (a A_1 : Tm m),
+                    Γ_1 ⊢ S type →
+                      eqM ▸ Γ ⬝ A = Γ_1 ⊗ Δ →
+                        eqM ▸ b = a →
+                          eqM ▸ B⌈(ₛidₚ), v(0), (A⌊↑ₚidₚ⌋.refl v(0))⌉ = A_1 → (Γ_1 ⬝ S ⊗ ⌊↑₁↬l⌋Δ) ⊢ a⌊↑₁m↬l⌋ ∶ A_1⌊↑₁m↬l⌋) →
+                  (∀ (m l : Nat) (Γ_1 : Ctx l) (Δ : CtxGen l m) (eqM : n = m) (S : Tm l) (a_6 A_1 : Tm m),
+                      Γ_1 ⊢ S type →
+                        eqM ▸ Γ = Γ_1 ⊗ Δ →
+                          eqM ▸ a = a_6 → eqM ▸ A = A_1 → (Γ_1 ⬝ S ⊗ ⌊↑₁↬l⌋Δ) ⊢ a_6⌊↑₁m↬l⌋ ∶ A_1⌊↑₁m↬l⌋) →
+                    (∀ (m l : Nat) (Γ_1 : Ctx l) (Δ : CtxGen l m) (eqM : n = m) (S : Tm l) (a A_1 : Tm m),
+                        Γ_1 ⊢ S type →
+                          eqM ▸ Γ = Γ_1 ⊗ Δ →
+                            eqM ▸ a' = a → eqM ▸ A = A_1 → (Γ_1 ⬝ S ⊗ ⌊↑₁↬l⌋Δ) ⊢ a⌊↑₁m↬l⌋ ∶ A_1⌊↑₁m↬l⌋) →
+                      (∀ (m l : Nat) (Γ_1 : Ctx l) (Δ : CtxGen l m) (eqM : n = m) (S : Tm l) (a_8 A_1 : Tm m),
+                          Γ_1 ⊢ S type →
+                            eqM ▸ Γ = Γ_1 ⊗ Δ →
+                              eqM ▸ p = a_8 → (eqM ▸ a ≃[A] a') = A_1 → (Γ_1 ⬝ S ⊗ ⌊↑₁↬l⌋Δ) ⊢ a_8⌊↑₁m↬l⌋ ∶ A_1⌊↑₁m↬l⌋) →
+                        ∀ (m l : Nat) (Γ_1 : Ctx l) (Δ : CtxGen l m) (eqM : n = m) (S : Tm l) (a_9 A_1 : Tm m),
+                          Γ_1 ⊢ S type →
+                            eqM ▸ Γ = Γ_1 ⊗ Δ →
+                              eqM ▸ A.j B b a a' p = a_9 →
+                                eqM ▸ B⌈(ₛidₚ), a, a', p⌉ = A_1 → (Γ_1 ⬝ S ⊗ ⌊↑₁↬l⌋Δ) ⊢ a_9⌊↑₁m↬l⌋ ∶ A_1⌊↑₁m↬l⌋ :=
+  by
+    intro n Γ A B b a a' p hB hbB haA haA' hpId ihB ihbB ihaA ihaA' ihpId
+    intro m l Γ Δ heqM S t T hS heqΓ heqt heqT
+    cases heqM
+    cases heqΓ
+    cases heqt
+    cases heqT
+    rw [weak_subst_iden_elim]
+    apply HasType.iden_elim
+    · have h := gen_ctx_leq Δ
+      simp [lift_weak_n]
+      rw [lift_weaken_from]
+      rw [lift_weaken_from]
+      rw [lift_weaken_from]
+      rw [←shift_weaken_from]
+      rw (config := {occs := .pos [2]}) [←weakening_shift_id]
+      rw [←shift_weaken_from]
+      rw [←shift_weaken_from]
+      rw [weakening_shift_id]
+      rw [←helper_weak_iden_propagate_weak]
+      rw [extend_expand_context_weaken_from]
+      rw [extend_expand_context_weaken_from]
+      rw [extend_expand_context_weaken_from]
+      apply ihB
+      apply hS
+      repeat' rfl
+      any_goals omega
+    · have h := gen_ctx_leq Δ
+      rw [extend_expand_context_weaken_from]
+      simp [lift_weak_n]
+      rw [lift_weaken_from]
+      rw [helper_weak_refl_propagate_weak]
+      apply ihbB
+      apply hS
+      repeat' rfl
+      any_goals omega
+    · apply ihaA
+      apply hS
+      repeat' rfl
+    · apply ihaA'
+      apply hS
+      repeat' rfl
+    · rw [←weakening_iden]
+      apply ihpId
+      apply hS
+      repeat' rfl
+
+theorem weakening_ty_conv :
+    ∀ {n : Nat} {Γ : Ctx n} {a A B : Tm n},
+      (Γ ⊢ a ∶ A) →
+        Γ ⊢ A ≡ B type →
+          (∀ (m l : Nat) (Γ_1 : Ctx l) (Δ : CtxGen l m) (eqM : n = m) (S : Tm l) (a_3 A_1 : Tm m),
+              Γ_1 ⊢ S type →
+                eqM ▸ Γ = Γ_1 ⊗ Δ → eqM ▸ a = a_3 → eqM ▸ A = A_1 → (Γ_1 ⬝ S ⊗ ⌊↑₁↬l⌋Δ) ⊢ a_3⌊↑₁m↬l⌋ ∶ A_1⌊↑₁m↬l⌋) →
+            (∀ (m l : Nat) (Γ_1 : Ctx l) (Δ : CtxGen l m) (eqM : n = m) (S : Tm l) (A_1 A' : Tm m),
+                Γ_1 ⊢ S type →
+                  eqM ▸ Γ = Γ_1 ⊗ Δ → eqM ▸ A = A_1 → eqM ▸ B = A' → (Γ_1 ⬝ S ⊗ ⌊↑₁↬l⌋Δ) ⊢ A_1⌊↑₁m↬l⌋ ≡ A'⌊↑₁m↬l⌋ type) →
+              ∀ (m l : Nat) (Γ_1 : Ctx l) (Δ : CtxGen l m) (eqM : n = m) (S : Tm l) (a_5 A : Tm m),
+                Γ_1 ⊢ S type → eqM ▸ Γ = Γ_1 ⊗ Δ → eqM ▸ a = a_5 → eqM ▸ B = A → (Γ_1 ⬝ S ⊗ ⌊↑₁↬l⌋Δ) ⊢ a_5⌊↑₁m↬l⌋ ∶ A⌊↑₁m↬l⌋ :=
+  by
+    intro n Γ a A B haA hAB ihaA ihAB m l Γ Δ heqM S t T hS heqΓ heqt heqT
+    cases heqM
+    cases heqΓ
+    cases heqt
+    cases heqT
+    apply HasType.ty_conv
+    · apply ihaA
+      apply hS
+      repeat' rfl
+    · apply ihAB
+      apply hS
+      repeat' rfl
+
