IMLTT/typed/proofs/admissable/WeakeningAlt/IsType.lean
@@ -10,73 +10,173 @@ import IMLTT.typed.JudgmentsAndRules
 import IMLTT.typed.proofs.Recursor
 import IMLTT.typed.proofs.boundary.BoundaryIsCtx
 
--- case IsTypeUnitForm
--- ⊢ ∀ {n : Nat} {Γ : Ctx n},
---     Γ ctx →
---       (∀ (m l : Nat) (Γ_1 : Ctx l) (Δ : CtxGen l m) (eqM : n = m) (S : Tm l),
---           Γ_1 ⊢ S type → eqM ▸ Γ = Γ_1 ⊗ Δ → (Γ_1 ⬝ S ⊗ ⌊↑₁↬l⌋Δ) ctx) →
---         ∀ (m l : Nat) (Γ_1 : Ctx l) (Δ : CtxGen l m) (eqM : n = m) (S : Tm l) (A : Tm m),
---           Γ_1 ⊢ S type → eqM ▸ Γ = Γ_1 ⊗ Δ → eqM ▸ 𝟙 = A → (Γ_1 ⬝ S ⊗ ⌊↑₁↬l⌋Δ) ⊢ A⌊↑₁m↬l⌋ type
--- case IsTypeEmptyForm
--- ⊢ ∀ {n : Nat} {Γ : Ctx n},
---     Γ ctx →
---       (∀ (m l : Nat) (Γ_1 : Ctx l) (Δ : CtxGen l m) (eqM : n = m) (S : Tm l),
---           Γ_1 ⊢ S type → eqM ▸ Γ = Γ_1 ⊗ Δ → (Γ_1 ⬝ S ⊗ ⌊↑₁↬l⌋Δ) ctx) →
---         ∀ (m l : Nat) (Γ_1 : Ctx l) (Δ : CtxGen l m) (eqM : n = m) (S : Tm l) (A : Tm m),
---           Γ_1 ⊢ S type → eqM ▸ Γ = Γ_1 ⊗ Δ → eqM ▸ 𝟘 = A → (Γ_1 ⬝ S ⊗ ⌊↑₁↬l⌋Δ) ⊢ A⌊↑₁m↬l⌋ type
--- case IsTypePiForm
--- ⊢ ∀ {n : Nat} {Γ : Ctx n} {A : Tm n} {B : Tm (n + 1)},
---     Γ ⊢ A type →
---       Γ ⬝ A ⊢ B type →
---         (∀ (m l : Nat) (Γ_1 : Ctx l) (Δ : CtxGen l m) (eqM : n = m) (S : Tm l) (A_1 : Tm m),
---             Γ_1 ⊢ S type → eqM ▸ Γ = Γ_1 ⊗ Δ → eqM ▸ A = A_1 → (Γ_1 ⬝ S ⊗ ⌊↑₁↬l⌋Δ) ⊢ A_1⌊↑₁m↬l⌋ type) →
---           (∀ (m l : Nat) (Γ_1 : Ctx l) (Δ : CtxGen l m) (eqM : n + 1 = m) (S : Tm l) (A_1 : Tm m),
---               Γ_1 ⊢ S type → eqM ▸ Γ ⬝ A = Γ_1 ⊗ Δ → eqM ▸ B = A_1 → (Γ_1 ⬝ S ⊗ ⌊↑₁↬l⌋Δ) ⊢ A_1⌊↑₁m↬l⌋ type) →
---             ∀ (m l : Nat) (Γ_1 : Ctx l) (Δ : CtxGen l m) (eqM : n = m) (S : Tm l) (A_1 : Tm m),
---               Γ_1 ⊢ S type → eqM ▸ Γ = Γ_1 ⊗ Δ → (eqM ▸ ΠA;B) = A_1 → (Γ_1 ⬝ S ⊗ ⌊↑₁↬l⌋Δ) ⊢ A_1⌊↑₁m↬l⌋ type
--- case IsTypeSigmaForm
--- ⊢ ∀ {n : Nat} {Γ : Ctx n} {A : Tm n} {B : Tm (n + 1)},
---     Γ ⊢ A type →
---       Γ ⬝ A ⊢ B type →
---         (∀ (m l : Nat) (Γ_1 : Ctx l) (Δ : CtxGen l m) (eqM : n = m) (S : Tm l) (A_1 : Tm m),
---             Γ_1 ⊢ S type → eqM ▸ Γ = Γ_1 ⊗ Δ → eqM ▸ A = A_1 → (Γ_1 ⬝ S ⊗ ⌊↑₁↬l⌋Δ) ⊢ A_1⌊↑₁m↬l⌋ type) →
---           (∀ (m l : Nat) (Γ_1 : Ctx l) (Δ : CtxGen l m) (eqM : n + 1 = m) (S : Tm l) (A_1 : Tm m),
---               Γ_1 ⊢ S type → eqM ▸ Γ ⬝ A = Γ_1 ⊗ Δ → eqM ▸ B = A_1 → (Γ_1 ⬝ S ⊗ ⌊↑₁↬l⌋Δ) ⊢ A_1⌊↑₁m↬l⌋ type) →
---             ∀ (m l : Nat) (Γ_1 : Ctx l) (Δ : CtxGen l m) (eqM : n = m) (S : Tm l) (A_1 : Tm m),
---               Γ_1 ⊢ S type → eqM ▸ Γ = Γ_1 ⊗ Δ → (eqM ▸ ΣA;B) = A_1 → (Γ_1 ⬝ S ⊗ ⌊↑₁↬l⌋Δ) ⊢ A_1⌊↑₁m↬l⌋ type
--- case IsTypeNatForm
--- ⊢ ∀ {n : Nat} {Γ : Ctx n},
---     Γ ctx →
---       (∀ (m l : Nat) (Γ_1 : Ctx l) (Δ : CtxGen l m) (eqM : n = m) (S : Tm l),
---           Γ_1 ⊢ S type → eqM ▸ Γ = Γ_1 ⊗ Δ → (Γ_1 ⬝ S ⊗ ⌊↑₁↬l⌋Δ) ctx) →
---         ∀ (m l : Nat) (Γ_1 : Ctx l) (Δ : CtxGen l m) (eqM : n = m) (S : Tm l) (A : Tm m),
---           Γ_1 ⊢ S type → eqM ▸ Γ = Γ_1 ⊗ Δ → eqM ▸ 𝒩 = A → (Γ_1 ⬝ S ⊗ ⌊↑₁↬l⌋Δ) ⊢ A⌊↑₁m↬l⌋ type
--- case IsTypeIdenForm
--- ⊢ ∀ {n : Nat} {Γ : Ctx n} {a A a' : Tm n},
---     Γ ⊢ A type →
---       (Γ ⊢ a ∶ A) →
---         (Γ ⊢ a' ∶ A) →
---           (∀ (m l : Nat) (Γ_1 : Ctx l) (Δ : CtxGen l m) (eqM : n = m) (S : Tm l) (A_1 : Tm m),
---               Γ_1 ⊢ S type → eqM ▸ Γ = Γ_1 ⊗ Δ → eqM ▸ A = A_1 → (Γ_1 ⬝ S ⊗ ⌊↑₁↬l⌋Δ) ⊢ A_1⌊↑₁m↬l⌋ type) →
---             (∀ (m l : Nat) (Γ_1 : Ctx l) (Δ : CtxGen l m) (eqM : n = m) (S : Tm l) (a_5 A_1 : Tm m),
---                 Γ_1 ⊢ S type →
---                   eqM ▸ Γ = Γ_1 ⊗ Δ → eqM ▸ a = a_5 → eqM ▸ A = A_1 → (Γ_1 ⬝ S ⊗ ⌊↑₁↬l⌋Δ) ⊢ a_5⌊↑₁m↬l⌋ ∶ A_1⌊↑₁m↬l⌋) →
---               (∀ (m l : Nat) (Γ_1 : Ctx l) (Δ : CtxGen l m) (eqM : n = m) (S : Tm l) (a A_1 : Tm m),
---                   Γ_1 ⊢ S type →
---                     eqM ▸ Γ = Γ_1 ⊗ Δ → eqM ▸ a' = a → eqM ▸ A = A_1 → (Γ_1 ⬝ S ⊗ ⌊↑₁↬l⌋Δ) ⊢ a⌊↑₁m↬l⌋ ∶ A_1⌊↑₁m↬l⌋) →
---                 ∀ (m l : Nat) (Γ_1 : Ctx l) (Δ : CtxGen l m) (eqM : n = m) (S : Tm l) (A_1 : Tm m),
---                   Γ_1 ⊢ S type → eqM ▸ Γ = Γ_1 ⊗ Δ → (eqM ▸ a ≃[A] a') = A_1 → (Γ_1 ⬝ S ⊗ ⌊↑₁↬l⌋Δ) ⊢ A_1⌊↑₁m↬l⌋ type
--- case IsTypeUnivForm
--- ⊢ ∀ {n : Nat} {Γ : Ctx n},
---     Γ ctx →
---       (∀ (m l : Nat) (Γ_1 : Ctx l) (Δ : CtxGen l m) (eqM : n = m) (S : Tm l),
---           Γ_1 ⊢ S type → eqM ▸ Γ = Γ_1 ⊗ Δ → (Γ_1 ⬝ S ⊗ ⌊↑₁↬l⌋Δ) ctx) →
---         ∀ (m l : Nat) (Γ_1 : Ctx l) (Δ : CtxGen l m) (eqM : n = m) (S : Tm l) (A : Tm m),
---           Γ_1 ⊢ S type → eqM ▸ Γ = Γ_1 ⊗ Δ → eqM ▸ 𝒰 = A → (Γ_1 ⬝ S ⊗ ⌊↑₁↬l⌋Δ) ⊢ A⌊↑₁m↬l⌋ type
--- case IsTypeUnivElim
--- ⊢ ∀ {n : Nat} {Γ : Ctx n} {A : Tm n},
---     (Γ ⊢ A ∶ 𝒰) →
---       (∀ (m l : Nat) (Γ_1 : Ctx l) (Δ : CtxGen l m) (eqM : n = m) (S : Tm l) (a A_1 : Tm m),
---           Γ_1 ⊢ S type → eqM ▸ Γ = Γ_1 ⊗ Δ → eqM ▸ A = a → eqM ▸ 𝒰 = A_1 → (Γ_1 ⬝ S ⊗ ⌊↑₁↬l⌋Δ) ⊢ a⌊↑₁m↬l⌋ ∶ A_1⌊↑₁m↬l⌋) →
---         ∀ (m l : Nat) (Γ_1 : Ctx l) (Δ : CtxGen l m) (eqM : n = m) (S : Tm l) (A_1 : Tm m),
---           Γ_1 ⊢ S type → eqM ▸ Γ = Γ_1 ⊗ Δ → eqM ▸ A = A_1 → (Γ_1 ⬝ S ⊗ ⌊↑₁↬l⌋Δ) ⊢ A_1⌊↑₁m↬l⌋ type
+theorem weakening_unit_form :
+    ∀ {n : Nat} {Γ : Ctx n},
+      Γ ctx →
+        (∀ (m l : Nat) (Γ_1 : Ctx l) (Δ : CtxGen l m) (eqM : n = m) (S : Tm l),
+            Γ_1 ⊢ S type → eqM ▸ Γ = Γ_1 ⊗ Δ → (Γ_1 ⬝ S ⊗ ⌊↑₁↬l⌋Δ) ctx) →
+          ∀ (m l : Nat) (Γ_1 : Ctx l) (Δ : CtxGen l m) (eqM : n = m) (S : Tm l) (A : Tm m),
+            Γ_1 ⊢ S type → eqM ▸ Γ = Γ_1 ⊗ Δ → eqM ▸ 𝟙 = A → (Γ_1 ⬝ S ⊗ ⌊↑₁↬l⌋Δ) ⊢ A⌊↑₁m↬l⌋ type :=
+  by
+    intro n Γ' hiC ihiC m l Γ Δ heqM S T hS heqΓ heqt
+    cases heqM
+    cases heqΓ
+    cases heqt
+    apply IsType.unit_form
+    apply ihiC
+    apply hS
+    repeat' rfl
+
+theorem weakening_empty_form :
+    ∀ {n : Nat} {Γ : Ctx n},
+      Γ ctx →
+        (∀ (m l : Nat) (Γ_1 : Ctx l) (Δ : CtxGen l m) (eqM : n = m) (S : Tm l),
+            Γ_1 ⊢ S type → eqM ▸ Γ = Γ_1 ⊗ Δ → (Γ_1 ⬝ S ⊗ ⌊↑₁↬l⌋Δ) ctx) →
+          ∀ (m l : Nat) (Γ_1 : Ctx l) (Δ : CtxGen l m) (eqM : n = m) (S : Tm l) (A : Tm m),
+            Γ_1 ⊢ S type → eqM ▸ Γ = Γ_1 ⊗ Δ → eqM ▸ 𝟘 = A → (Γ_1 ⬝ S ⊗ ⌊↑₁↬l⌋Δ) ⊢ A⌊↑₁m↬l⌋ type :=
+  by
+    intro n Γ' hiC ihiC m l Γ Δ heqM S T hS heqΓ heqt
+    cases heqM
+    cases heqΓ
+    cases heqt
+    apply IsType.empty_form
+    apply ihiC
+    apply hS
+    repeat' rfl
+
+theorem weakening_pi_form :
+    ∀ {n : Nat} {Γ : Ctx n} {A : Tm n} {B : Tm (n + 1)},
+      Γ ⊢ A type →
+        Γ ⬝ A ⊢ B type →
+          (∀ (m l : Nat) (Γ_1 : Ctx l) (Δ : CtxGen l m) (eqM : n = m) (S : Tm l) (A_1 : Tm m),
+              Γ_1 ⊢ S type → eqM ▸ Γ = Γ_1 ⊗ Δ → eqM ▸ A = A_1 → (Γ_1 ⬝ S ⊗ ⌊↑₁↬l⌋Δ) ⊢ A_1⌊↑₁m↬l⌋ type) →
+            (∀ (m l : Nat) (Γ_1 : Ctx l) (Δ : CtxGen l m) (eqM : n + 1 = m) (S : Tm l) (A_1 : Tm m),
+                Γ_1 ⊢ S type → eqM ▸ Γ ⬝ A = Γ_1 ⊗ Δ → eqM ▸ B = A_1 → (Γ_1 ⬝ S ⊗ ⌊↑₁↬l⌋Δ) ⊢ A_1⌊↑₁m↬l⌋ type) →
+              ∀ (m l : Nat) (Γ_1 : Ctx l) (Δ : CtxGen l m) (eqM : n = m) (S : Tm l) (A_1 : Tm m),
+                Γ_1 ⊢ S type → eqM ▸ Γ = Γ_1 ⊗ Δ → (eqM ▸ ΠA;B) = A_1 → (Γ_1 ⬝ S ⊗ ⌊↑₁↬l⌋Δ) ⊢ A_1⌊↑₁m↬l⌋ type :=
+  by
+    intro n Γ' A B hA hB ihA ihB m l Γ Δ heqM S T hS heqΓ heqT
+    cases heqM
+    cases heqΓ
+    cases heqT
+    apply IsType.pi_form
+    · apply ihA
+      apply hS
+      repeat' rfl
+    · simp [extend_expand_context_weaken_from]
+      simp [lift_weak_n]
+      rw [lift_weaken_from]
+      apply ihB
+      apply hS
+      repeat' rfl
+      apply gen_ctx_leq Δ
+
+theorem weakening_sigma_form :
+    ∀ {n : Nat} {Γ : Ctx n} {A : Tm n} {B : Tm (n + 1)},
+      Γ ⊢ A type →
+        Γ ⬝ A ⊢ B type →
+          (∀ (m l : Nat) (Γ_1 : Ctx l) (Δ : CtxGen l m) (eqM : n = m) (S : Tm l) (A_1 : Tm m),
+              Γ_1 ⊢ S type → eqM ▸ Γ = Γ_1 ⊗ Δ → eqM ▸ A = A_1 → (Γ_1 ⬝ S ⊗ ⌊↑₁↬l⌋Δ) ⊢ A_1⌊↑₁m↬l⌋ type) →
+            (∀ (m l : Nat) (Γ_1 : Ctx l) (Δ : CtxGen l m) (eqM : n + 1 = m) (S : Tm l) (A_1 : Tm m),
+                Γ_1 ⊢ S type → eqM ▸ Γ ⬝ A = Γ_1 ⊗ Δ → eqM ▸ B = A_1 → (Γ_1 ⬝ S ⊗ ⌊↑₁↬l⌋Δ) ⊢ A_1⌊↑₁m↬l⌋ type) →
+              ∀ (m l : Nat) (Γ_1 : Ctx l) (Δ : CtxGen l m) (eqM : n = m) (S : Tm l) (A_1 : Tm m),
+                Γ_1 ⊢ S type → eqM ▸ Γ = Γ_1 ⊗ Δ → (eqM ▸ ΣA;B) = A_1 → (Γ_1 ⬝ S ⊗ ⌊↑₁↬l⌋Δ) ⊢ A_1⌊↑₁m↬l⌋ type :=
+  by
+    intro n Γ' A B hA hB ihA ihB m l Γ Δ heqM S T hS heqΓ heqT
+    cases heqM
+    cases heqΓ
+    cases heqT
+    apply IsType.sigma_form
+    · apply ihA
+      apply hS
+      repeat' rfl
+    · simp [extend_expand_context_weaken_from]
+      simp [lift_weak_n]
+      rw [lift_weaken_from]
+      apply ihB
+      apply hS
+      repeat' rfl
+      apply gen_ctx_leq Δ
+
+theorem weakening_nat_form :
+    ∀ {n : Nat} {Γ : Ctx n},
+      Γ ctx →
+        (∀ (m l : Nat) (Γ_1 : Ctx l) (Δ : CtxGen l m) (eqM : n = m) (S : Tm l),
+            Γ_1 ⊢ S type → eqM ▸ Γ = Γ_1 ⊗ Δ → (Γ_1 ⬝ S ⊗ ⌊↑₁↬l⌋Δ) ctx) →
+          ∀ (m l : Nat) (Γ_1 : Ctx l) (Δ : CtxGen l m) (eqM : n = m) (S : Tm l) (A : Tm m),
+            Γ_1 ⊢ S type → eqM ▸ Γ = Γ_1 ⊗ Δ → eqM ▸ 𝒩 = A → (Γ_1 ⬝ S ⊗ ⌊↑₁↬l⌋Δ) ⊢ A⌊↑₁m↬l⌋ type :=
+  by
+    intro n Γ' hiC ihiC m l Γ Δ heqM S T hS heqΓ heqt
+    cases heqM
+    cases heqΓ
+    cases heqt
+    apply IsType.nat_form
+    apply ihiC
+    apply hS
+    repeat' rfl
+
+theorem weakening_iden_form :
+    ∀ {n : Nat} {Γ : Ctx n} {a A a' : Tm n},
+      Γ ⊢ A type →
+        (Γ ⊢ a ∶ A) →
+          (Γ ⊢ a' ∶ A) →
+            (∀ (m l : Nat) (Γ_1 : Ctx l) (Δ : CtxGen l m) (eqM : n = m) (S : Tm l) (A_1 : Tm m),
+                Γ_1 ⊢ S type → eqM ▸ Γ = Γ_1 ⊗ Δ → eqM ▸ A = A_1 → (Γ_1 ⬝ S ⊗ ⌊↑₁↬l⌋Δ) ⊢ A_1⌊↑₁m↬l⌋ type) →
+              (∀ (m l : Nat) (Γ_1 : Ctx l) (Δ : CtxGen l m) (eqM : n = m) (S : Tm l) (a_5 A_1 : Tm m),
+                  Γ_1 ⊢ S type →
+                    eqM ▸ Γ = Γ_1 ⊗ Δ → eqM ▸ a = a_5 → eqM ▸ A = A_1 → (Γ_1 ⬝ S ⊗ ⌊↑₁↬l⌋Δ) ⊢ a_5⌊↑₁m↬l⌋ ∶ A_1⌊↑₁m↬l⌋) →
+                (∀ (m l : Nat) (Γ_1 : Ctx l) (Δ : CtxGen l m) (eqM : n = m) (S : Tm l) (a A_1 : Tm m),
+                    Γ_1 ⊢ S type →
+                      eqM ▸ Γ = Γ_1 ⊗ Δ → eqM ▸ a' = a → eqM ▸ A = A_1 → (Γ_1 ⬝ S ⊗ ⌊↑₁↬l⌋Δ) ⊢ a⌊↑₁m↬l⌋ ∶ A_1⌊↑₁m↬l⌋) →
+                  ∀ (m l : Nat) (Γ_1 : Ctx l) (Δ : CtxGen l m) (eqM : n = m) (S : Tm l) (A_1 : Tm m),
+                    Γ_1 ⊢ S type → eqM ▸ Γ = Γ_1 ⊗ Δ → (eqM ▸ a ≃[A] a') = A_1 → (Γ_1 ⬝ S ⊗ ⌊↑₁↬l⌋Δ) ⊢ A_1⌊↑₁m↬l⌋ type :=
+  by
+    intro n Γ' a A a' hA haA haA' ihA ihaA ihaA' m l Γ Δ heqM S T hS heqΓ heqT
+    cases heqM
+    cases heqΓ
+    cases heqT
+    apply IsType.iden_form
+    · apply ihA
+      apply hS
+      repeat' rfl
+    · apply ihaA
+      apply hS
+      repeat' rfl
+    · apply ihaA'
+      apply hS
+      repeat' rfl
+
+theorem weakening_univ_form :
+    ∀ {n : Nat} {Γ : Ctx n},
+      Γ ctx →
+        (∀ (m l : Nat) (Γ_1 : Ctx l) (Δ : CtxGen l m) (eqM : n = m) (S : Tm l),
+            Γ_1 ⊢ S type → eqM ▸ Γ = Γ_1 ⊗ Δ → (Γ_1 ⬝ S ⊗ ⌊↑₁↬l⌋Δ) ctx) →
+          ∀ (m l : Nat) (Γ_1 : Ctx l) (Δ : CtxGen l m) (eqM : n = m) (S : Tm l) (A : Tm m),
+            Γ_1 ⊢ S type → eqM ▸ Γ = Γ_1 ⊗ Δ → eqM ▸ 𝒰 = A → (Γ_1 ⬝ S ⊗ ⌊↑₁↬l⌋Δ) ⊢ A⌊↑₁m↬l⌋ type :=
+  by
+    intro n Γ' hiC ihiC m l Γ Δ heqM S T hS heqΓ heqt
+    cases heqM
+    cases heqΓ
+    cases heqt
+    apply IsType.univ_form
+    apply ihiC
+    apply hS
+    repeat' rfl
+
+theorem weakening_univ_elim :
+    ∀ {n : Nat} {Γ : Ctx n} {A : Tm n},
+      (Γ ⊢ A ∶ 𝒰) →
+        (∀ (m l : Nat) (Γ_1 : Ctx l) (Δ : CtxGen l m) (eqM : n = m) (S : Tm l) (a A_1 : Tm m),
+            Γ_1 ⊢ S type → eqM ▸ Γ = Γ_1 ⊗ Δ → eqM ▸ A = a → eqM ▸ 𝒰 = A_1 → (Γ_1 ⬝ S ⊗ ⌊↑₁↬l⌋Δ) ⊢ a⌊↑₁m↬l⌋ ∶ A_1⌊↑₁m↬l⌋) →
+          ∀ (m l : Nat) (Γ_1 : Ctx l) (Δ : CtxGen l m) (eqM : n = m) (S : Tm l) (A_1 : Tm m),
+            Γ_1 ⊢ S type → eqM ▸ Γ = Γ_1 ⊗ Δ → eqM ▸ A = A_1 → (Γ_1 ⬝ S ⊗ ⌊↑₁↬l⌋Δ) ⊢ A_1⌊↑₁m↬l⌋ type :=
+  by
+    intro n Γ A hAU ihAU m l Γ Δ heqM S T hS heqΓ heqT
+    cases heqM
+    cases heqΓ
+    cases heqT
+    apply IsType.univ_elim
+    rw [←weakening_univ]
+    apply ihAU
+    apply hS
+    repeat' rfl
