IMLTT/typed/proofs/admissable/WeakeningAlt/Weakening.lean
@@ -1,0 +1,268 @@
+import IMLTT.untyped.AbstractSyntax
+import IMLTT.untyped.Weakening
+import IMLTT.untyped.Substitution
+import IMLTT.untyped.proofs.Weakening
+import IMLTT.untyped.proofs.Substitution
+import IMLTT.untyped.proofs.Contexts
+import IMLTT.untyped.proofs.Mixture
+
+import IMLTT.typed.JudgmentsAndRules
+import IMLTT.typed.proofs.Recursor
+import IMLTT.typed.proofs.boundary.BoundaryIsCtx
+
+import IMLTT.typed.proofs.admissable.weakeningalt.IsCtx
+import IMLTT.typed.proofs.admissable.weakeningalt.IsType
+import IMLTT.typed.proofs.admissable.weakeningalt.HasType
+import IMLTT.typed.proofs.admissable.weakeningalt.IsEqualType
+import IMLTT.typed.proofs.admissable.weakeningalt.IsEqualTerm
+
+theorem weakening :
+  (∀ {n l : Nat} {Γ : Ctx l} {Δ : CtxGen l n} {S : Tm l},
+    (Γ ⊗ Δ) ctx → (Γ ⊢ S type)
+    → (Γ ⬝ S ⊗ (⌊↑₁↬l⌋Δ) ctx)) ∧
+  (∀ {n l : Nat} {Γ : Ctx l} {Δ : CtxGen l n} {A : Tm n} {S : Tm l},
+    (Γ ⊗ Δ) ⊢ A type → (Γ ⊢ S type)
+    → (Γ ⬝ S ⊗ (⌊↑₁↬l⌋Δ)) ⊢ A⌊↑₁n↬l⌋ type) ∧
+  (∀ {n l : Nat} {Γ : Ctx l} {Δ : CtxGen l n} {A a : Tm n} {S : Tm l},
+    ((Γ ⊗ Δ) ⊢ a ∶ A) → (Γ ⊢ S type)
+    → (Γ ⬝ S ⊗ (⌊↑₁↬l⌋Δ)) ⊢ a⌊↑₁n↬l⌋ ∶ A⌊↑₁n↬l⌋) ∧
+  (∀ {n l : Nat} {Γ : Ctx l} {Δ : CtxGen l n} {A A' : Tm n} {S : Tm l},
+    (Γ ⊗ Δ) ⊢ A ≡ A' type → (Γ ⊢ S type)
+    → (Γ ⬝ S ⊗ (⌊↑₁↬l⌋Δ)) ⊢ A⌊↑₁n↬l⌋ ≡ A'⌊↑₁n↬l⌋ type) ∧
+  (∀ {n l : Nat} {Γ : Ctx l} {Δ : CtxGen l n} {A a a' : Tm n} {S : Tm l},
+    ((Γ ⊗ Δ) ⊢ a ≡ a' ∶ A) → (Γ ⊢ S type)
+    → (Γ ⬝ S ⊗ (⌊↑₁↬l⌋Δ)) ⊢ a⌊↑₁n↬l⌋ ≡ a'⌊↑₁n↬l⌋ ∶ A⌊↑₁n↬l⌋) :=
+  by
+    suffices h :
+        (∀ {n : Nat} {Γ : Ctx n},
+      Γ ctx →
+        ∀ (m l : Nat) (Γ_1 : Ctx l) (Δ : CtxGen l m) (eqM : n = m) (S : Tm l),
+          Γ_1 ⊢ S type → eqM ▸ Γ = Γ_1 ⊗ Δ → (Γ_1 ⬝ S ⊗ ⌊↑₁↬l⌋Δ) ctx) ∧
+    (∀ {n : Nat} {Γ : Ctx n} {A : Tm n},
+        Γ ⊢ A type →
+          ∀ (m l : Nat) (Γ_1 : Ctx l) (Δ : CtxGen l m) (eqM : n = m) (S : Tm l) (A_1 : Tm m),
+            Γ_1 ⊢ S type → eqM ▸ Γ = Γ_1 ⊗ Δ → eqM ▸ A = A_1 → (Γ_1 ⬝ S ⊗ ⌊↑₁↬l⌋Δ) ⊢ A_1⌊↑₁m↬l⌋ type) ∧
+      (∀ {n : Nat} {Γ : Ctx n} {A a : Tm n},
+          (Γ ⊢ a ∶ A) →
+            ∀ (m l : Nat) (Γ_1 : Ctx l) (Δ : CtxGen l m) (eqM : n = m) (S : Tm l) (a_1 A_1 : Tm m),
+              Γ_1 ⊢ S type →
+                eqM ▸ Γ = Γ_1 ⊗ Δ → eqM ▸ a = a_1 → eqM ▸ A = A_1 → (Γ_1 ⬝ S ⊗ ⌊↑₁↬l⌋Δ) ⊢ a_1⌊↑₁m↬l⌋ ∶ A_1⌊↑₁m↬l⌋) ∧
+        (∀ {n : Nat} {Γ : Ctx n} {A A' : Tm n},
+            Γ ⊢ A ≡ A' type →
+              ∀ (m l : Nat) (Γ_1 : Ctx l) (Δ : CtxGen l m) (eqM : n = m) (S : Tm l) (A_1 A'_1 : Tm m),
+                Γ_1 ⊢ S type →
+                  eqM ▸ Γ = Γ_1 ⊗ Δ →
+                    eqM ▸ A = A_1 → eqM ▸ A' = A'_1 → (Γ_1 ⬝ S ⊗ ⌊↑₁↬l⌋Δ) ⊢ A_1⌊↑₁m↬l⌋ ≡ A'_1⌊↑₁m↬l⌋ type) ∧
+          ∀ {n : Nat} {Γ : Ctx n} {A a a' : Tm n},
+            (Γ ⊢ a ≡ a' ∶ A) →
+              ∀ (m l : Nat) (Γ_1 : Ctx l) (Δ : CtxGen l m) (eqM : n = m) (S : Tm l) (a_1 a'_1 A_1 : Tm m),
+                Γ_1 ⊢ S type →
+                  eqM ▸ Γ = Γ_1 ⊗ Δ →
+                    eqM ▸ a = a_1 →
+                      eqM ▸ a' = a'_1 → eqM ▸ A = A_1 → (Γ_1 ⬝ S ⊗ ⌊↑₁↬l⌋Δ) ⊢ a_1⌊↑₁m↬l⌋ ≡ a'_1⌊↑₁m↬l⌋ ∶ A_1⌊↑₁m↬l⌋
+      by
+        any_goals repeat' (apply And.intro)
+        · intro n l Γ Δ S hiC hS
+          apply (And.left h)
+          · apply hiC
+          · apply hS
+          · rfl
+          · rfl
+        · intro n l Γ Δ A S hA hS
+          apply And.left (And.right h)
+          · apply hA
+          · apply hS
+          · rfl
+          · rfl
+          · rfl
+        · intro n l Γ Δ A a S haA hS
+          apply And.left (And.right (And.right h))
+          · apply haA
+          · apply hS
+          · rfl
+          · rfl
+          · rfl
+          · rfl
+        · intro n l Γ Δ A A' S hAA hS
+          apply And.left (And.right (And.right (And.right h)))
+          · apply hAA
+          · apply hS
+          · rfl
+          · rfl
+          · rfl
+          · rfl
+        · intro n l Γ Δ A a a' S haaA hS
+          apply And.right (And.right (And.right (And.right h)))
+          · apply haaA
+          · apply hS
+          · rfl
+          · rfl
+          · rfl
+          · rfl
+          · rfl
+    apply judgment_recursor
+      (motive_1 := fun {n} Γ' _hiC =>
+        ∀ m l (Γ : Ctx l) (Δ : CtxGen l m) (eqM : n = m) S,
+        (Γ ⊢ S type)
+        → eqM ▸ Γ' = (Γ ⊗ Δ)
+        → (Γ ⬝ S ⊗ (⌊↑₁↬l⌋Δ)) ctx)
+      (motive_2 := fun {n} Γ' A' _hA =>
+        ∀ m l (Γ : Ctx l) (Δ : CtxGen l m) (eqM : n = m) S A,
+        (Γ ⊢ S type)
+        → eqM ▸ Γ' = (Γ ⊗ Δ) → eqM ▸ A' = A
+        → (Γ ⬝ S ⊗ (⌊↑₁↬l⌋Δ)) ⊢ A⌊↑₁m↬l⌋ type)
+      (motive_3 := fun {n} Γ' a' A' haA =>
+        ∀ m l (Γ : Ctx l) (Δ : CtxGen l m) (eqM : n = m) S a A,
+        (Γ ⊢ S type)
+        → eqM ▸ Γ' = (Γ ⊗ Δ) → eqM ▸ a' = a → eqM ▸ A' = A
+        → (Γ ⬝ S ⊗ (⌊↑₁↬l⌋Δ)) ⊢ (a⌊↑₁m↬l⌋) ∶ (A⌊↑₁m↬l⌋))
+      (motive_4 := fun {n} Γ' C C' _hCC =>
+        ∀ m l (Γ : Ctx l) (Δ : CtxGen l m) (eqM : n = m) S A A',
+        (Γ ⊢ S type)
+        → eqM ▸ Γ' = (Γ ⊗ Δ) → eqM ▸ C = A → eqM ▸ C' = A'
+        → (Γ ⬝ S ⊗ (⌊↑₁↬l⌋Δ)) ⊢ (A⌊↑₁m↬l⌋) ≡ (A'⌊↑₁m↬l⌋) type)
+      (motive_5 := fun {n} Γ' c c' C _haaA => 
+        ∀ m l (Γ : Ctx l) (Δ : CtxGen l m) (eqM : n = m) S a a' A,
+        (Γ ⊢ S type)
+        → eqM ▸ Γ' = (Γ ⊗ Δ) → eqM ▸ c = a → eqM ▸ c' = a' → eqM ▸ C = A
+        → (Γ ⬝ S ⊗ (⌊↑₁↬l⌋Δ)) ⊢ (a⌊↑₁m↬l⌋) ≡ (a'⌊↑₁m↬l⌋) ∶ (A⌊↑₁m↬l⌋))
+    case IsCtxEmpty =>
+      apply weakening_gen_empty
+    case IsCtxExtend =>
+      apply weakening_gen_extend
+    case IsTypeUnitForm =>
+      apply weakening_unit_form
+    case IsTypeEmptyForm =>
+      apply weakening_empty_form
+    case IsTypePiForm =>
+      apply weakening_pi_form
+    case IsTypeSigmaForm =>
+      apply weakening_sigma_form
+    case IsTypeNatForm =>
+      apply weakening_nat_form
+    case IsTypeIdenForm =>
+      apply weakening_iden_form
+    case IsTypeUnivForm =>
+      apply weakening_univ_form
+    case IsTypeUnivElim =>
+      apply weakening_univ_elim
+    case HasTypeVar =>
+      apply weakening_var
+    case HasTypeWeak =>
+      apply weakening_weak
+    case HasTypeUnitIntro =>
+      apply weakening_unit_intro
+    case HasTypePiIntro =>
+      apply weakening_pi_intro
+    case HasTypeSigmaIntro =>
+      apply weakening_sigma_intro
+    case HasTypeNatZeroIntro =>
+      apply weakening_nat_zero_intro
+    case HasTypeNatSuccIntro =>
+      apply weakening_nat_succ_intro
+    case HasTypeIdenIntro =>
+      apply weakening_iden_intro
+    case HasTypeUnivUnit =>
+      apply weakening_univ_unit
+    case HasTypeUnivEmpty =>
+      apply weakening_univ_empty
+    case HasTypeUnivPi =>
+      apply weakening_univ_pi
+    case HasTypeUnivSigma =>
+      apply weakening_univ_sigma
+    case HasTypeUnivNat =>
+      apply weakening_univ_nat
+    case HasTypeUnivIden =>
+      apply weakening_univ_iden
+    case HasTypeUnitElim =>
+      apply weakening_unit_elim
+    case HasTypeEmptyElim =>
+      apply weakening_empty_elim
+    case HasTypePiElim =>
+      apply weakening_pi_elim
+    case HasTypeSigmaElim =>
+      apply weakening_sigma_elim
+    case HasTypeNatElim =>
+      apply weakening_nat_elim
+    case HasTypeIdenElim =>
+      apply weakening_iden_elim
+    case HasTypeTyConv =>
+      apply weakening_ty_conv
+    case IsEqualTypeUnitFormEq =>
+      apply weakening_unit_form_eq
+    case IsEqualTypeEmptyFormEq =>
+      apply weakening_empty_form_eq
+    case IsEqualTypePiFormEq =>
+      apply weakening_pi_form_eq
+    case IsEqualTypeSigmaFormEq =>
+      apply weakening_sigma_form_eq
+    case IsEqualTypeNatFormEq =>
+      apply weakening_nat_form_eq
+    case IsEqualTypeIdenFormEq =>
+      apply weakening_iden_form_eq
+    case IsEqualTypeUnivFormEq =>
+      apply weakening_univ_form_eq
+    case IsEqualTypeUnivElimEq =>
+      apply weakening_univ_elim_eq
+    case IsEqualTypeTypeSymm =>
+      apply weakening_type_symm
+    case IsEqualTypeTypeTrans =>
+      apply weakening_type_trans
+    case IsEqualTermVarEq =>
+      apply weakening_var_eq
+    case IsEqualTermWeakEq =>
+      apply weakening_weak_eq
+    case IsEqualTermUnitComp =>
+      apply weakening_unit_comp
+    case IsEqualTermPiComp =>
+      apply weakening_pi_comp
+    case IsEqualTermSigmaComp =>
+      apply weakening_sigma_comp
+    case IsEqualTermNatZeroComp =>
+      apply weakening_nat_zero_comp
+    case IsEqualTermNatSuccComp =>
+      apply weakening_nat_succ_comp
+    case IsEqualTermIdenComp =>
+      apply weakening_iden_comp
+    case IsEqualTermUnitIntroEq =>
+      apply weakening_unit_intro_eq
+    case IsEqualTermUnitElimEq =>
+      apply weakening_unit_elim_eq
+    case IsEqualTermEmptyElimEq =>
+      apply weakening_empty_elim_eq
+    case IsEqualTermPiIntroEq =>
+      apply weakening_pi_intro_eq
+    case IsEqualTermPiElimEq =>
+      apply weakening_pi_elim_eq
+    case IsEqualTermSigmaIntroEq =>
+      apply weakening_sigma_intro_eq
+    case IsEqualTermSigmaElimEq =>
+      apply weakening_sigma_elim_eq
+    case IsEqualTermNatZeroIntroEq =>
+      apply weakening_nat_zero_intro_eq
+    case IsEqualTermNatSuccIntroEq =>
+      apply weakening_nat_succ_intro_eq
+    case IsEqualTermNatElimEq =>
+      apply weakening_nat_elim_eq
+    case IsEqualTermIdenIntroEq =>
+      apply weakening_iden_intro_eq
+    case IsEqualTermIdenElimEq =>
+      apply weakening_iden_elim_eq
+    case IsEqualTermUnivUnitEq =>
+      apply weakening_univ_unit_eq
+    case IsEqualTermUnivEmptyEq =>
+      apply weakening_univ_empty_eq
+    case IsEqualTermUnivPiEq =>
+      apply weakening_univ_pi_eq
+    case IsEqualTermUnivSigmaEq =>
+      apply weakening_univ_sigma_eq
+    case IsEqualTermUnivNatEq =>
+      apply weakening_univ_nat_eq
+    case IsEqualTermUnivIdenEq =>
+      apply weakening_univ_iden_eq
+    case IsEqualTermTyConvEq =>
+      apply weakening_ty_conv_eq
+    case IsEqualTermTermSymm =>
+      apply weakening_term_symm
+    case IsEqualTermTermTrans =>
+      apply weakening_term_trans
