IMLTT/untyped/proofs/Substitution.lean
@@ -103,12 +103,20 @@ theorem substitution_var_substitute {σ σ' : Subst m n} :
       apply And.intro
       · apply substitution_var_substitute h
       · apply substitution_var_substitute h
-    | .firstSigma p =>
+    | .indSigma A B C c p =>
       simp [substitute]
-      apply substitution_var_substitute h
-    | .secondSigma p =>
-      simp [substitute]
-      apply substitution_var_substitute h
+      apply And.intro
+      · apply substitution_var_substitute h
+      · apply And.intro
+        · apply substitution_var_substitute
+          apply substitution_var_lift h
+        · apply And.intro
+          · apply substitution_var_substitute
+            apply substitution_var_lift h
+          · apply And.intro
+            · apply substitution_var_substitute
+              apply substitution_var_lift_n h
+            · apply substitution_var_substitute h
     | .zeroNat =>
       simp [substitute]
     | .succNat x =>
@@ -248,12 +256,29 @@ theorem substitution_id {t : Tm n} :
       apply And.intro
       · apply substitution_id
       · apply substitution_id
-    | .firstSigma p =>
+    | .indSigma A B C c p =>
       simp [substitute]
-      apply substitution_id
-    | .secondSigma p =>
-      simp [substitute]
-      apply substitution_id
+      apply And.intro
+      · apply substitution_id
+      · apply And.intro
+        · have h := substitution_id (t := B)
+          rw (config := {occs := .pos [2]}) [←h]
+          apply substitution_var_substitute
+          intro x
+          apply substitution_var_lift_n_id
+        · apply And.intro
+          · have h := substitution_id (t := C)
+            rw (config := {occs := .pos [2]}) [←h]
+            apply substitution_var_substitute
+            intro x
+            apply substitution_var_lift_n_id
+          · apply And.intro
+            · have h := substitution_id (t := c)
+              rw (config := {occs := .pos [2]}) [←h]
+              apply substitution_var_substitute
+              intro x
+              apply substitution_var_lift_n_id
+            · apply substitution_id
     | .zeroNat =>
       simp [substitute]
     | .succNat i =>
